Reorganised files

Compiler.v
@@ -1,1530 +1,789 @@
-Require Import String.
-Require Import Bool Arith Omega List Coq.Program.Equality.
-Require Import Maps Imp.
-Require Import Sequences Semantics.
-
-
-
-(** This chapter defines a compiler from the Imp language to a virtual machine
-  (a small subset of the Java Virtual Machine) and proves that this
-  compiler preserves the semantics of the source programs. *)
-
-(** * 1. The virtual machine. *)
-
-(** The machine operates on a code [c] (a fixed list of instructions)
-  and three variable components:
-- a program counter, denoting a position in [c]
-- a state assigning integer values to variables
-- an evaluation stack, containing integers.
-*)
-
-(** The instruction set of the machine. *)
-
-Inductive instruction: Type :=
-  | Iconst(n: nat)                 (**r push integer [n] on stack *)
-  | Ivar(x: id)                    (**r push the value of variable [x] *)
-  | Isetvar(x: id)                 (**r pop an integer, assign it to variable [x] *)
-  | Iadd                           (**r pop [n2], pop [n1], push back [n1+n2] *)
-  | Isub                           (**r pop [n2], pop [n1], push back [n1-n2] *)
-  | Imul                           (**r pop [n2], pop [n1], push back [n1*n2] *)
-  | Ibranch_forward(ofs: nat)      (**r skip [ofs] instructions forward *)
-  | Ibranch_backward(ofs: nat)     (**r skip [ofs] instructions backward *)
-  | Ibeq(ofs: nat)                 (**r pop [n2], pop [n1], skip [ofs] forward if [n1=n2] *)
-  | Ibne(ofs: nat)                 (**r pop [n2], pop [n1], skip [ofs] forward if [n1<>n2] *)
-  | Ible(ofs: nat)                 (**r pop [n2], pop [n1], skip [ofs] forward if [n1<=n2] *)
-  | Ibgt(ofs: nat)                 (**r pop [n2], pop [n1], skip [ofs] forward if [n1>n2] *)
-  | Ihalt.                         (**r terminate execution successfully *)
-
-Definition code := list instruction.
-
-(** [code_at C pc = Some i] if [i] is the instruction at position [pc]
-  in the list of instructions [C]. *)
-
-Fixpoint code_at (C: code) (pc: nat) : option instruction :=
-  match C, pc with
-  | nil, _ => None
-  | i :: C', O => Some i
-  | i :: C', S pc' => code_at C' pc'
-  end.
-
-Definition stack := list nat.
-
-(** The semantics of the virtual machine is given in small-step style,
-  as a transition relation between machine configuration: triples
-  (program counter, evaluation stack, variable state).
-  The transition relation is parameterized by the code [c].
-  There is one transition rule for each kind of instruction,
-  except [Ihalt], which has no transition. *)
-
-Definition configuration := (nat * stack * state)%type.
-
-Inductive transition (C: code): configuration -> configuration -> Prop :=
-  | trans_const: forall pc stk s n,
-      code_at C pc = Some(Iconst n) ->
-      transition C (pc, stk, s) (pc + 1, n :: stk, s)
-  | trans_var: forall pc stk s x,
-      code_at C pc = Some(Ivar x) ->
-      transition C (pc, stk, s) (pc + 1, s x :: stk, s)
-  | trans_setvar: forall pc stk s x n,
-      code_at C pc = Some(Isetvar x) ->
-      transition C (pc, n :: stk, s) (pc + 1, stk, t_update s x n)
-  | trans_add: forall pc stk s n1 n2,
-      code_at C pc = Some(Iadd) ->
-      transition C (pc, n2 :: n1 :: stk, s) (pc + 1, (n1 + n2) :: stk, s)
-  | trans_sub: forall pc stk s n1 n2,
-      code_at C pc = Some(Isub) ->
-      transition C (pc, n2 :: n1 :: stk, s) (pc + 1, (n1 - n2) :: stk, s)
-  | trans_mul: forall pc stk s n1 n2,
-      code_at C pc = Some(Imul) ->
-      transition C (pc, n2 :: n1 :: stk, s) (pc + 1, (n1 * n2) :: stk, s)
-  | trans_branch_forward: forall pc stk s ofs pc',
-      code_at C pc = Some(Ibranch_forward ofs) ->
-      pc' = pc + 1 + ofs ->
-      transition C (pc, stk, s) (pc', stk, s)
-  | trans_branch_backward: forall pc stk s ofs pc',
-      code_at C pc = Some(Ibranch_backward ofs) ->
-      pc' = pc + 1 - ofs ->
-      transition C (pc, stk, s) (pc', stk, s)
-  | trans_beq: forall pc stk s ofs n1 n2 pc',
-      code_at C pc = Some(Ibeq ofs) ->
-      pc' = (if beq_nat n1 n2 then pc + 1 + ofs else pc + 1) ->
-      transition C (pc, n2 :: n1 :: stk, s) (pc', stk, s)
-  | trans_bne: forall pc stk s ofs n1 n2 pc',
-      code_at C pc = Some(Ibne ofs) ->
-      pc' = (if beq_nat n1 n2 then pc + 1 else pc + 1 + ofs) ->
-      transition C (pc, n2 :: n1 :: stk, s) (pc', stk, s)
-  | trans_ble: forall pc stk s ofs n1 n2 pc',
-      code_at C pc = Some(Ible ofs) ->
-      pc' = (if leb n1 n2 then pc + 1 + ofs else pc + 1) ->
-      transition C (pc, n2 :: n1 :: stk, s) (pc', stk, s)
-  | trans_bgt: forall pc stk s ofs n1 n2 pc',
-      code_at C pc = Some(Ibgt ofs) ->
-      pc' = (if leb n1 n2 then pc + 1 else pc + 1 + ofs) ->
-      transition C (pc, n2 :: n1 :: stk, s) (pc', stk, s).
-
-(** As usual with small-step semantics, we form sequences of machine transitions
-  to define the behavior of a code.  We always start with [pc = 0]
-  and an empty evaluation stack.  We stop successfully if [pc] points
-  to an [Ihalt] instruction and the evaluation stack is empty.
-
-  If [R] is a binary relation, [star R] is its reflexive transitive closure.
-  (See file [Sequences] for the definition.)  [star (transition C)]
-  therefore represents a sequence of  zero, one or several machine transitions.
-*)
-
-Definition mach_terminates (C: code) (s_init s_fin: state) :=
-  exists pc,
-  code_at C pc = Some Ihalt /\
-  star (transition C) (0, nil, s_init) (pc, nil, s_fin).
-
-(** Likewise, [infseq R] represents an infinite sequence of [R] transitions.
-  (Also defined in file [Sequences].) *)
-
-Definition mach_diverges (C: code) (s_init: state) :=
-  infseq (transition C) (0, nil, s_init).
-
-(** A third case can occur: after a finite number of transitions,
-  the machine hits a configuration where it cannot make any transition,
-  and this state is not a final configuration ([Ihalt] instruction and empty stack).
-  In this case, we say that the machine "goes wrong", which is
-  a politically-correct way of saying that our program just crashed. *)
-
-Definition mach_goes_wrong (C: code) (s_init: state) :=
-  exists pc, exists stk, exists s_fin,
-  star (transition C) (0, nil, s_init) (pc, stk, s_fin)
-  /\ irred (transition C) (pc, stk, s_fin)
-  /\ (code_at C pc <> Some Ihalt \/ stk <> nil).
-
-(** An important property of the virtual machine is that it is deterministic:
-  from a given configuration, it can transition to at most one other configuration. *)
-
-Lemma machine_deterministic:
-  forall C config config1 config2,
-  transition C config config1 -> transition C config config2 -> config1 = config2.
-Proof.
-  intros. inversion H; subst; inversion H0; try congruence.
-  destruct (beq_nat n1 n2); congruence.
-  destruct (beq_nat n1 n2); congruence.
-  destruct (leb n1 n2); congruence.
-  destruct (leb n1 n2); congruence.
-Qed.
-
-(** As a consequence of this determinism, it follows that
-  the final state of a terminating program is unique,
-  and that a program cannot both terminate and diverge,
-  or terminate and go wrong, or diverge and go wrong.
-  These results follow from the generic determinism properties 
-  found at the end of module [Sequence]. *)
-
-Remark stop_irred:
-  forall C pc stk st,
-  code_at C pc = Some Ihalt -> irred (transition C) (pc, stk, st).
-Proof.
-  unfold irred; intros. unfold not; intros. inversion H0; congruence.
-Qed.
-
-Lemma terminates_unique:
-  forall C st st1 st2, mach_terminates C st st1 -> mach_terminates C st st2 -> st1 = st2.
-Proof.
-  unfold mach_terminates; intros. destruct H as (pc1 & A1 & B1), H0 as (pc2 & A2 & B2).
-  assert (((pc1, nil, st1) : configuration) = ((pc2, nil, st2) : configuration)).
-  { eapply finseq_unique; eauto using machine_deterministic, stop_irred. }
-  congruence. 
-Qed.
-
-Lemma terminates_goeswrong_exclusive:
-  forall C st st', mach_terminates C st st' -> mach_goes_wrong C st -> False.
-Proof.
-  unfold mach_terminates, mach_goes_wrong; intros.
-  destruct H as (pc1 & A1 & B1), H0 as (pc2 & stk2 & st2 & A2 & B2 & C2).
-  assert (((pc1, nil, st') : configuration) = ((pc2, stk2, st2) : configuration)).
-  { eapply finseq_unique; eauto using machine_deterministic, stop_irred. }
-  inversion H. subst pc2 stk2 st2. destruct C2; congruence.
-Qed.
-
-Lemma terminates_diverges_exclusive:
-  forall C st st', mach_terminates C st st' -> mach_diverges C st -> False.
-Proof.
-  unfold mach_terminates, mach_diverges; intros.
-  destruct H as (pc1 & A1 & B1).
-  eapply infseq_finseq_excl with (R := transition C); eauto using machine_deterministic, stop_irred.
-Qed.
-
-Lemma goeswrong_diverges_exclusive:
-  forall C st, mach_goes_wrong C st -> mach_diverges C st -> False.
-Proof.
-  unfold mach_terminates, mach_diverges; intros. 
-  destruct H as (pc2 & stk2 & st2 & A2 & B2 & C2).
-  eapply infseq_finseq_excl with (R := transition C); eauto using machine_deterministic, stop_irred.
-Qed.
-
-(** *** Exercise (2 stars, recommended). *)
-(** To quickly see how a machine program executes, it is convenient
-  to redefine the semantics of the machine as an executable function
-  instead of inductively-defined relations.  This is similar to the
-  [ceval_step] function from the [Imp] chapter of Software Foundations,
-  which provides an executable interpreter for the Imp language.
-
-  To ensure termination of the machine interpreter, we need to bound 
-  the number of instructions it can execute.  The result of the
-  machine interpreter, therefore, is of the following type:
-*)
-
-Inductive machine_result : Type :=
-  | Timeout : machine_result              (**r the interpreter ran out of fuel *)
-  | GoesWrong : machine_result            (**r the machine goes wrong on an impossible case *)
-  | Terminates : state -> machine_result. (**r the machine successfully stops with the given state *)
-
-(** Please fill in the blanks in the following definition for a machine interpreter: *)
-
-Fixpoint mach_interp (C: code) (fuel: nat)
-                     (pc: nat) (stk: stack) (st: state) : machine_result :=
-  match fuel with
-  | O => Timeout
-  | S fuel' =>
-      match code_at C pc, stk with
-      | Some Ihalt, nil => Terminates st
-      | Some (Iconst n), stk => mach_interp C fuel' (pc + 1) (n :: stk) st
-      (* FILL IN HERE *)
-      | _, _ => GoesWrong
-      end
-  end.
-
-(** * 2. The compilation scheme *)
-
-(** The code for an arithmetic expression [a]
-- executes in sequence (no branches)
-- deposits the value of [a] at the top of the stack
-- preserves the variable state.
-
-This is the familiar translation to "reverse Polish notation".
- *)
-
-Locate "++".
-Open Scope list.
-Fixpoint compile_aexp (a: aexp) : code :=
-  match a with
-  | ANum n => Iconst n :: nil
-  | AId v => Ivar v :: nil
-  | APlus a1 a2 => compile_aexp a1 ++ compile_aexp a2 ++ Iadd :: nil
-  | AMinus a1 a2 => compile_aexp a1 ++ compile_aexp a2 ++ Isub :: nil
-  | AMult a1 a2 => compile_aexp a1 ++ compile_aexp a2 ++ Imul :: nil
-  end.
-
-(** Some examples. *)
-
-Notation vx := (Id "X").
-Notation vy := (Id "Y").
-
-Compute (compile_aexp (APlus (AId vx) (ANum 1))).
-
-(** Result is: [ [Ivar vx, Iconst 1, Iadd] ] *)
-
-Compute (compile_aexp (AMult (AId vy) (APlus (AId vx) (ANum 1)))).
-
-(** Result is: [ [Ivar vy, Ivar vx, Iconst 1, Iadd, Imul] ] *)
-
-(** The code [compile_bexp b cond ofs] for a boolean expression [b]
-- skips forward the [ofs] following instructions if [b] evaluates to [cond] (a boolean)
-- executes in sequence if [b] evaluates to the negation of [cond]
-- leaves the stack and the variable state unchanged.
-
-See slides for explanation of the mysterious branch offsets!
-*)
-
-Search "length".
-
-Fixpoint compile_bexp (b: bexp) (cond: bool) (ofs: nat) : code :=
-  match b with
-  | BTrue =>
-      if cond then Ibranch_forward ofs :: nil else nil
-  | BFalse =>
-      if cond then nil else Ibranch_forward ofs :: nil
-  | BEq a1 a2 =>
-      compile_aexp a1 ++ compile_aexp a2 ++
-      (if cond then Ibeq ofs :: nil else Ibne ofs :: nil)
-  | BLe a1 a2 =>
-      compile_aexp a1 ++ compile_aexp a2 ++
-      (if cond then Ible ofs :: nil else Ibgt ofs :: nil)
-  | BNot b1 =>
-      compile_bexp b1 (negb cond) ofs
-  | BAnd b1 b2 =>
-      let c2 := compile_bexp b2 cond ofs in
-      let c1 := compile_bexp b1 false (if cond then length c2 else ofs + length c2) in
-      (c1 ++ c2)%list
-  end.
-
-(** Examples. *)
-
-Compute (compile_bexp (BEq (AId vx) (ANum 1)) true 42).
-
-(** Result is: [ [Ivar vx, Iconst 1, Ibeq 42] ] *)
-
-Compute (compile_bexp (BAnd (BLe (ANum 1) (AId vx)) (BLe (AId vx) (ANum 10))) false 42).
-
-(** Result is: [ [Iconst 1, Ivar vx, Ibgt 45, Ivar vx, Iconst 10, Ibgt 42] ] *)
-
-Compute (compile_bexp (BNot (BAnd BTrue BFalse)) true 42).
-
-(** Result is: [ [Ibranch_forward 42] ] *)
-
-(** The code for a command [c]
-- updates the variable state as prescribed by [c]
-- preserves the stack
-- finishes on the next instruction immediately following the generated code.
-
-Again, see slides for explanations of the generated branch offsets.
-*)
-
-Fixpoint compile_com (c: com) : code :=
-  match c with
-  | SKIP =>
-      nil
-  | (id ::= a) =>
-      compile_aexp a ++ Isetvar id :: nil
-  | (c1 ;; c2) =>
-      compile_com c1 ++ compile_com c2
-  | IFB b THEN ifso ELSE ifnot FI =>
-      let code_ifso := compile_com ifso in
-      let code_ifnot := compile_com ifnot in
-      compile_bexp b false (length code_ifso + 1)
-      ++ code_ifso
-      ++ Ibranch_forward (length code_ifnot)
-      :: code_ifnot
-  | WHILE b DO body END =>
-      let code_body := compile_com body in
-      let code_test := compile_bexp b false (length code_body + 1) in
-      code_test
-      ++ code_body
-      ++ Ibranch_backward (length code_test + length code_body + 1)
-      :: nil
-  end.
-
-(** The code for a program [p] (a command) is similar, but terminates
-  cleanly on an [Ihalt] instruction. *)
-
-Definition compile_program (p: com) : code :=
-  compile_com p ++ Ihalt :: nil.
-
-(** Examples of compilation: *)
-
-Compute (compile_program (vx ::= APlus (AId vx) (ANum 1))).
-
-(** Result is: [ [Ivar vx, Iconst 1, Iadd, Isetvar vx, Ihalt] ] *)
-
-Compute (compile_program (WHILE BTrue DO SKIP END)).
-
-(** Result is: [ [Ibranch_backward 1, Ihalt] ].  That's a tight loop indeed! *)
-
-Compute (compile_program (IFB BEq (AId vx) (ANum 1) THEN vx ::= ANum 0 ELSE SKIP FI)).
-
-(** Result is: [ [Ivar vx, Iconst 1, Ibne 3, Iconst 0, Isetvar vx, Ibranch_forward 0, Ihalt] ] *)
-
-(** *** Exercise (1 star, recommended) *)
-(** The last example shows a slight inefficiency in the code generated for
-  [IFB ... THEN ... ELSE SKIP FI].  How would you change [compile_com]
-  to generate better code?  Hint: ponder the following function. *)
-
-Definition smart_Ibranch_forward (ofs: nat) : code :=
-  if beq_nat ofs 0 then nil else Ibranch_forward(ofs) :: nil.
-
-(** * 3. Semantic preservation *)
-
-(** ** Auxiliary results about code sequences. *)
-
-(** To reason about the execution of compiled code, we need to consider
-  code sequences [C2] that are at position [pc] in a bigger code
-  sequence [C = C1 ++ C2 ++ C3].  The following predicate
-  [codeseq_at C pc C2] does just this. *)
-
-Inductive codeseq_at: code -> nat -> code -> Prop :=
-  | codeseq_at_intro: forall C1 C2 C3 pc,
-      pc = length C1 ->
-      codeseq_at (C1 ++ C2 ++ C3) pc C2.
-
-(** We show a number of no-brainer lemmas about [code_at] and [codeseq_at],
-  then populate a "hint database" so that Coq can use them automatically. *)
-
-Lemma code_at_app:
-  forall i c2 c1 pc,
-  pc = length c1 ->
-  code_at (c1 ++ i :: c2) pc = Some i.
-Proof.
-  induction c1; simpl; intros; subst pc; auto.
-Qed.
-
-Lemma codeseq_at_head:
-  forall C pc i C',
-  codeseq_at C pc (i :: C') ->
-  code_at C pc = Some i.
-Proof.
-  intros. inversion H. simpl. apply code_at_app. auto.
-Qed.
-
-Lemma codeseq_at_tail:
-  forall C pc i C',
-  codeseq_at C pc (i :: C') ->
-  codeseq_at C (pc + 1) C'.
-Proof.
-  intros. inversion H. 
-  change (C1 ++ (i :: C') ++ C3)
-    with (C1 ++ (i :: nil) ++ C' ++ C3).
-  rewrite <- app_ass. constructor. rewrite app_length. auto.
-Qed. 
-
-Lemma codeseq_at_app_left:
-  forall C pc C1 C2,
-  codeseq_at C pc (C1 ++ C2) ->
-  codeseq_at C pc C1.
-Proof.
-  intros. inversion H. rewrite app_ass. constructor. auto.
-Qed.
-
-Lemma codeseq_at_app_right:
-  forall C pc C1 C2,
-  codeseq_at C pc (C1 ++ C2) ->
-  codeseq_at C (pc + length C1) C2.
-Proof.
-  intros. inversion H. rewrite app_ass. rewrite <- app_ass. constructor. rewrite app_length. auto.
-Qed.
-
-Lemma codeseq_at_app_right2:
-  forall C pc C1 C2 C3,
-  codeseq_at C pc (C1 ++ C2 ++ C3) ->
-  codeseq_at C (pc + length C1) C2.
-Proof.
-  intros. inversion H. repeat rewrite app_ass. rewrite <- app_ass. constructor. rewrite app_length. auto.
-Qed.
-
-Hint Resolve codeseq_at_head codeseq_at_tail codeseq_at_app_left codeseq_at_app_right codeseq_at_app_right2: codeseq.
+Set Warnings "-notation-overridden,-parsing".
+From Coq Require Import Strings.String.
+From Coq Require Import Bool.Bool.
+From Coq Require Import Arith.Arith.
+From Coq Require Import Lists.List.
+From StorelessMachine Require Import Sequences.
+From StorelessMachine Require Import Maps.
+From StorelessMachine Require Import Imp.
+From StorelessMachine Require Import Facts.
+Require Import Omega.
 
 Ltac normalize :=
   repeat rewrite app_length in *;
   repeat rewrite plus_assoc in *;
   repeat rewrite plus_0_r in *;
+  repeat rewrite Nat.sub_0_r in *;
   simpl in *.
 
-(** ** Correctness of generated code for expressions. *)
-
-(** Remember the informal specification we gave for the code generated
-  for an arithmetic expression [a].  It should
-- execute in sequence (no branches)
-- deposit the value of [a] at the top of the stack
-- preserve the variable state.
-
-We now prove that the code [compile_aexp a] fulfills this contract.
-The proof is a nice induction on the structure of [a]. *)
-
-Lemma compile_aexp_correct:
-  forall C st a pc stk,
-  codeseq_at C pc (compile_aexp a) ->
-  star (transition C)
-       (pc, stk, st)
-       (pc + length (compile_aexp a), aeval st a :: stk, st).
-Proof.
-  induction a; simpl; intros.
-
-- (* ANum *)
-  apply star_one. apply trans_const. eauto with codeseq. 
-
-- (* AId *)
-  apply star_one. apply trans_var. eauto with codeseq. 
-
-- (* APlus *)
-  eapply star_trans.
-  apply IHa1. eauto with codeseq. 
-  eapply star_trans.
-  apply IHa2. eauto with codeseq. 
-  apply star_one. normalize. apply trans_add. eauto with codeseq. 
-
-- (* AMinus *)
-  eapply star_trans.
-  apply IHa1. eauto with codeseq. 
-  eapply star_trans.
-  apply IHa2. eauto with codeseq. 
-  apply star_one. normalize. apply trans_sub. eauto with codeseq. 
-
-- (* AMult *)
-  eapply star_trans.
-  apply IHa1. eauto with codeseq. 
-  eapply star_trans.
-  apply IHa2. eauto with codeseq. 
-  apply star_one. normalize. apply trans_mul. eauto with codeseq. 
-Qed.
-
-(** Here is a similar proof for the compilation of boolean expressions. *)
-
-Lemma compile_bexp_correct:
-  forall C st b cond ofs pc stk,
-  codeseq_at C pc (compile_bexp b cond ofs) ->
-  star (transition C)
-       (pc, stk, st)
-       (pc + length (compile_bexp b cond ofs) + if eqb (beval st b) cond then ofs else 0, stk, st).
-Proof.
-  induction b; simpl; intros.
-
-- (* BTrue *)
-  destruct cond; simpl.
-  + (* BTrue, true *)
-    apply star_one. apply trans_branch_forward with ofs. eauto with codeseq. auto.
-  + (* BTrue, false *)
-    repeat rewrite plus_0_r. apply star_refl.
- 
-- (* BFalse *)
-  destruct cond; simpl.
-  + (* BFalse, true *)
-    repeat rewrite plus_0_r. apply star_refl.
-  + (* BFalse, false *)
-    apply star_one. apply trans_branch_forward with ofs. eauto with codeseq. auto.
-
-- (* BEq *)
-  eapply star_trans. 
-  apply compile_aexp_correct with (a := a). eauto with codeseq. 
-  eapply star_trans.
-  apply compile_aexp_correct with (a := a0). eauto with codeseq. 
-  apply star_one. normalize.
-  destruct cond.
-  + (* BEq, true *)
-    apply trans_beq with ofs. eauto with codeseq.
-    destruct (beq_nat (aeval st a) (aeval st a0)); simpl; omega.
-  + (* BEq, false *)
-    apply trans_bne with ofs. eauto with codeseq. 
-    destruct (beq_nat (aeval st a) (aeval st a0)); simpl; omega.
-
-- (* BLe *)
-  eapply star_trans. 
-  apply compile_aexp_correct with (a := a). eauto with codeseq. 
-  eapply star_trans.
-  apply compile_aexp_correct with (a := a0). eauto with codeseq. 
-  apply star_one. normalize.
-  destruct cond.
-  + (* BLe, true *)
-    apply trans_ble with ofs. eauto with codeseq.
-    destruct (leb (aeval st a) (aeval st a0)); simpl; omega.
-  + (* BLe, false *)
-    apply trans_bgt with ofs. eauto with codeseq. 
-    destruct (leb (aeval st a) (aeval st a0)); simpl; omega.
-
-- (* BNot *)
-  replace (eqb (negb (beval st b)) cond)
-     with (eqb (beval st b) (negb cond)).
-  apply IHb; auto. 
-  destruct (beval st b); destruct cond; auto.
-
-- (* BAnd *)
-  set (code_b2 := compile_bexp b2 cond ofs) in *.
-  set (ofs' := if cond then length code_b2 else ofs + length code_b2) in *.
-  set (code_b1 := compile_bexp b1 false ofs') in *.
-  apply star_trans with (pc + length code_b1 + (if eqb (beval st b1) false then ofs' else 0), stk, st).
-  apply IHb1. eauto with codeseq.
-  destruct cond.
-  + (* BAnd, true *)
-    destruct (beval st b1); simpl.
-    * (* b1 evaluates to true *)
-      normalize. apply IHb2. eauto with codeseq. 
-    * (* b1 evaluates to false *)
-      normalize. apply star_refl.
-  + (* BAnd, false *)
-    destruct (beval st b1); simpl.
-    * (* b1 evaluates to true *)
-      normalize. apply IHb2. eauto with codeseq. 
-    * (* b1 evaluates to false *)
-      replace ofs' with (length code_b2 + ofs). normalize. apply star_refl.
-      unfold ofs'; omega.
-Qed.
-
-(** ** Correctness of generated code for commands: terminating case. *)
-
-Lemma compile_com_correct_terminating:
-  forall C st c st',
-  c / st \\ st' ->
-  forall stk pc,
-  codeseq_at C pc (compile_com c) ->
-  star (transition C)
-       (pc, stk, st)
-       (pc + length (compile_com c), stk, st').
-Proof.
-  induction 1; intros stk pc AT.
-
-- (* SKIP *)
-  simpl in *. rewrite plus_0_r. apply star_refl.
-
-- (* := *)
-  simpl in *. subst n.
-  eapply star_trans. apply compile_aexp_correct. eauto with codeseq.
-  apply star_one. normalize. apply trans_setvar. eauto with codeseq. 
-
-- (* sequence *)
+Ltac normalize2 :=
+  repeat rewrite app_length in *;
+  repeat rewrite plus_assoc in *;
+  repeat rewrite plus_0_r in *;
+  repeat rewrite Nat.sub_0_r in *;
+  repeat rewrite Nat.add_1_r in *;
+  repeat rewrite Nat.add_0_r in *;
   simpl in *.
-  eapply star_trans. apply IHceval1. eauto with codeseq. 
-  normalize. apply IHceval2. eauto with codeseq. 
 
-- (* if true *)
-  simpl in *.
-  set (code1 := compile_com c1) in *.
-  set (codeb := compile_bexp b false (length code1 + 1)) in *.
-  set (code2 := compile_com c2) in *.
-  eapply star_trans. 
-  apply compile_bexp_correct with (b := b) (cond := false) (ofs := length code1 + 1).
-  eauto with codeseq. 
-  rewrite H. simpl. rewrite plus_0_r. fold codeb. normalize.
-  eapply star_trans. apply IHceval. eauto with codeseq. 
-  apply star_one. eapply trans_branch_forward. eauto with codeseq. omega.
 
-- (* if false *)
-  simpl in *.
-  set (code1 := compile_com c1) in *.
-  set (codeb := compile_bexp b false (length code1 + 1)) in *.
-  set (code2 := compile_com c2) in *.
-  eapply star_trans. 
-  apply compile_bexp_correct with (b := b) (cond := false) (ofs := length code1 + 1).
-  eauto with codeseq. 
-  rewrite H. simpl. fold codeb. normalize.
-  replace (pc + length codeb + length code1 + S(length code2))
-     with (pc + length codeb + length code1 + 1 + length code2).
-  apply IHceval. eauto with codeseq. omega. 
-
-- (* while false *)
-  simpl in *. 
-  eapply star_trans.
-  apply compile_bexp_correct with (b := b) (cond := false) (ofs := length (compile_com c) + 1). 
-  eauto with codeseq.
-  rewrite H. simpl. normalize. apply star_refl.
-
-- (* while true *)
-  apply star_trans with (pc, stk, st').
-  simpl in *.
-  eapply star_trans.
-  apply compile_bexp_correct with (b := b) (cond := false) (ofs := length (compile_com c) + 1). 
-  eauto with codeseq. 
-  rewrite H; simpl. rewrite plus_0_r.
-  eapply star_trans. apply IHceval1. eauto with codeseq. 
-  apply star_one.
-  eapply trans_branch_backward. eauto with codeseq. omega.
-  apply IHceval2. auto.
-Qed.
-
-Theorem compile_program_correct_terminating:
-  forall c st st',
-  c / st \\ st' ->
-  mach_terminates (compile_program c) st st'.
-Proof.
-  intros. unfold compile_program. red.
-  exists (length (compile_com c)); split.
-  apply code_at_app. auto.
-  apply compile_com_correct_terminating with (pc := 0). auto. 
-  apply codeseq_at_intro with (C1 := nil). auto.
-Qed.
-
-
-(** *** Exercise (2 stars, recommended) *)
-(** The previous exercise in this chapter suggested to use
-  [smart_Ibranch_forward] to avoid generating useless "branch forward"
-  instructions when compiling [IFB ... THEN ... ELSE SKIP FI] commands.
-  Once you have modified [compile_com] to use [smart_Ibranch_forward],
-  adapt the proof of [compile_com_correct_terminating] accordingly.
-  The following lemma will come handy: *)
-
-Lemma trans_smart_branch_forward:
-  forall C ofs pc stk st,
-  codeseq_at C pc (smart_Ibranch_forward ofs) ->
-  star (transition C) (pc, stk, st) (pc + length (smart_Ibranch_forward ofs) + ofs, stk, st).
-Proof.
-  unfold smart_Ibranch_forward; intros.
-  (* FILL IN HERE *)
-Admitted.
-
-(** *** Exercise (3 stars, optional) *)
-(** The manufacturer of our virtual machine offers a cheaper variant
-  that lacks the [Ibge] and [Ibgt] conditional branches.  The only
-  conditional branches available are [Ibeq] (branch if equal) and 
-  [Ibne] (branch if different).  Modify the definition of [compile_bexp] and
-  its correctness proof to target this cheaper virtual machine.
-  Hint: study Coq's definition of subtraction between natural numbers
-  (do [Print Nat.sub]). *)
-
-(** ** Correctness of generated code for commands: general case. *)
-
-(** We would like to strengthen the correctness result above so that it
-  is not restricted to terminating source programs, but also applies to
-  source program that diverge.  To this end, we abandon the big-step
-  semantics for commands and switch to the small-step semantics with continuations.
-  We then show a simulation theorem, establishing that every transition
-  of the small-step semantics in the source program is simulated (in a sense
-  to be made precise below) by zero, one or several transitions of the
-  machine executing the compiled code for the source program. *)
-
-(** Our first task is to relate configurations [(c, k, st)] of the small-step
-  semantics with configurations [(C, pc, stk, st)] of the machine.
-  We already know how to relate a command [c] with the machine code,
-  using the [codeseq_at] predicate.  What needs to be defined is a relation
-  between the continuation [k] and the machine code.
-
-  Intuitively, when the machine finishes executing the generated code for
-  command [c], that is, when it reaches the program point
-  [pc + length(compile_com c)], the machine should continue by executing
-  instructions that perform the pending computations described by
-  continuation [k], then reach an [Ihalt] instruction to stop cleanly.
-
-  We formalize this intution by the following inductive predicate
-  [compile_cont C k pc], which states that, starting at program point [pc],
-  there are instructions that perform the computations described in [k]
-  and reach an [Ihalt] instruction. *)
-
-Inductive compile_cont (C: code): cont -> nat -> Prop :=
-  | ccont_stop: forall pc,
-      code_at C pc = Some Ihalt ->
-      compile_cont C Kstop pc
-  | ccont_seq: forall c k pc pc',
-      codeseq_at C pc (compile_com c) ->
-      pc' = pc + length (compile_com c) ->
-      compile_cont C k pc' ->
-      compile_cont C (Kseq c k) pc
-  | ccont_while: forall b c k pc ofs pc' pc'',
-      code_at C pc = Some(Ibranch_backward ofs) ->
-      pc' = pc + 1 - ofs ->
-      codeseq_at C pc' (compile_com (WHILE b DO c END)) ->
-      pc'' = pc' + length (compile_com (WHILE b DO c END)) ->
-      compile_cont C k pc'' ->
-      compile_cont C (Kwhile b c k) pc
-  | ccont_branch: forall ofs k pc pc',
-      code_at C pc = Some(Ibranch_forward ofs) ->
-      pc' = pc + 1 + ofs ->
-      compile_cont C k pc' ->
-      compile_cont C k pc.
-
-(** Then, a configuration [(c,k,st)] of the small-step semantics matches
-  a configuration [(C, pc, stk, st')] of the machine if the following conditions hold:
-- The memory states are identical: [st' = st].
-- The machine stack is empty: [stk = nil].
-- The machine code at point [pc] is the compiled code for [c]:
-  [codeseq_at C pc (compile_com c)].
-- The machine code at point [pc + length (compile_com c)] matches continuation
-  [k], in the sense of [compile_cont] above.
-*)
-
-Inductive match_config (C: code): com * cont * state -> configuration -> Prop :=
-  | match_config_intro: forall c k st pc,
-      codeseq_at C pc (compile_com c) ->
-      compile_cont C k (pc + length (compile_com c)) ->
-      match_config C (c, k, st) (pc, nil, st).
-
-(** We are now ready to prove the expected simulation property.  Our first
-  attempt is to show a diagram of the following form:
-<<
-                      match_config
-     c / k / st  ----------------------- machstate
-       |                                   |
-       |                                   | *
-       |                                   |
-       v                                   v
-    c' / k' / st' ----------------------- machstate'
-                      match_config 
->>
-Hypotheses:
-- Left: one transition in the small-step continuation semantics for Imp.
-- Top: the [match_config] invariant.
-
-Conclusions:
-- Bottom: the [match_config] invariant, which must be preserved.
-- Right: zero, one or several transitions of the virtual machine.
-
-Why "zero, one, or several"?  Some transitions of the Imp semantics involve
-the evaluation of a complex expression, which requires several machine instructions
-to be executed.  However, other transitions of the Imp semantics, such as
-the [KS_Seq] and [KS_SkipSeq] rules, just change the focus on a sub-command,
-but the machine need not execute any instruction to reflect this change of focus.
-*)
-
-Lemma simulation_step_first_attempt:
-  forall C impstate1 impstate2 machstate1,
-  kstep impstate1 impstate2 ->
-  match_config C impstate1 machstate1 ->
-  exists machstate2,
-      star (transition C) machstate1 machstate2
-   /\ match_config C impstate2 machstate2.
-Proof.
-Abort.
-
-(** This simulation lemma is true and can be proved, but it is too weak to
-  imply the preservation of diverging behaviors: we have an issue with
-  "infinite stuttering".  Imagine a situation where the source program
-  takes infinitely many transitions, but every such transition is matched
-  by zero transitions of the virtual machine.  In this case, the source
-  program diverges, but the machine code can do anything: it can diverge,
-  as expected, but it can also terminate cleanly or go wrong. 
-  The simulation lemma above is too weak to rule out the last two cases!
-
-  We therefore need a stronger simulation result that rules out stuttering.
-  To this end, we are going to require that if a source transition is
-  matched by zero machine transition, some nonnegative measure of the source
-  configuration must strictly decrease.  This ensures that only a finite
-  number of stuttering steps can be taken before the machine actually does
-  a transition.  Here is the revised simulation diagram:
- 
-<<
-                      match_config
-     c / k / st  ----------------------- machconfig
-       |                                   |
-       |                                   | + or ( * and |c',k'| < |c,k} )
-       |                                   |
-       v                                   v
-    c' / k' / st' ----------------------- machconfig'
-                      match_config 
->>
-Note the stronger conclusion on the right:
-- either the virtual machine does one or several transitions
-- or it does zero, one or several transitions, but the size of the [c,k]
-  pair decreases strictly.
-
-It would be equivalent to state:
-- either the virtual machine does one or several transitions
-- or it does zero transitions, but the size of the [c,k] pair decreases strictly.
-
-However, the formulation above, with the "star" case, is often more convenient.
-*)
-
-(** Finding an appropriate "anti-stuttering" measure is a bit of a black art.
-After trial and error, we find that the following measure works.  It is
-the sum of the sizes of the command [c] under focus and all the commands
-appearing in the continuation [k]. *)
-
-Fixpoint com_size (c: com) : nat :=
-  match c with
-  | SKIP => 1
-  | x ::= a => 1
-  | (c1 ;; c2) => com_size c1 + com_size c2 + 1
-  | IFB b THEN ifso ELSE ifnot FI => com_size ifso + com_size ifnot + 1
-  | WHILE b DO c1 END => com_size c1 + 1
-  end.
-
-Remark com_size_nonzero: forall c, com_size c > 0. 
-Proof.
-  induction c; simpl; omega.
-Qed.
-
-Fixpoint cont_size (k: cont) : nat :=
-  match k with
-  | Kstop => 0
-  | Kseq c k' => com_size c + cont_size k'
-  | Kwhile b c k' => cont_size k'
-  end.
-
-Definition measure (impconf: com * cont * state) : nat :=
-  match impconf with (c, k, m) => com_size c + cont_size k end.
-
-(** A few technical lemmas to help with the simulation proof. *)
-
-Lemma compile_cont_Kstop_inv:
-  forall C pc m,
-  compile_cont C Kstop pc ->
-  exists pc',
-  star (transition C) (pc, nil, m) (pc', nil, m)
-  /\ code_at C pc' = Some Ihalt.
-Proof.
-  intros. dependent induction H. 
-- exists pc; split. apply star_refl. auto.
-- destruct IHcompile_cont as [pc'' [A B]]; auto.
-  exists pc''; split; auto. eapply star_step; eauto. eapply trans_branch_forward; eauto. 
-Qed.
-
-Lemma compile_cont_Kseq_inv:
-  forall C c k pc m,
-  compile_cont C (Kseq c k) pc ->
-  exists pc',
-  star (transition C) (pc, nil, m) (pc', nil, m)
-  /\ codeseq_at C pc' (compile_com c)
-  /\ compile_cont C k (pc' + length(compile_com c)).
-Proof.
-  intros. dependent induction H. 
-  exists pc; split. apply star_refl. split; congruence. 
-  destruct (IHcompile_cont _ _ eq_refl) as [pc'' [A [B D]]].
-  exists pc''; split; auto. eapply star_step; eauto. eapply trans_branch_forward; eauto. 
-Qed.
-
-Lemma compile_cont_Kwhile_inv:
-  forall C b c k pc m,
-  compile_cont C (Kwhile b c k) pc ->
-  exists pc',
-  plus (transition C) (pc, nil, m) (pc', nil, m)
-  /\ codeseq_at C pc' (compile_com (WHILE b DO c END))
-  /\ compile_cont C k (pc' + length(compile_com (WHILE b DO c END))).
-Proof.
-  intros. dependent induction H.
-- exists (pc + 1 - ofs); split.
-  apply plus_one. eapply trans_branch_backward; eauto. 
-  split; congruence.
-- destruct (IHcompile_cont _ _ _ (refl_equal _)) as [pc'' [A [B D]]].
-  exists pc''; split; auto. eapply plus_left. eapply trans_branch_forward; eauto. apply plus_star; auto. 
-Qed.
-
-Remark code_at_inv:
-  forall C pc i, code_at C pc = Some i -> exists C1, exists C2, C = C1 ++ C2 /\ length C1 = pc.
-Proof.
-  induction C; simpl; intros.
-  inversion H.
-  destruct pc. inversion H. exists (@nil instruction); exists (i :: C); auto. 
-  destruct (IHC _ _ H) as [C1 [C2 [A B]]].
-  exists (a :: C1); exists C2; split. simpl; congruence. simpl; congruence.
-Qed.
-
-Remark code_at_codeseq:
-  forall C pc i, code_at C pc = Some i -> codeseq_at C pc nil.
-Proof.
-  intros. destruct (code_at_inv _ _ _ H) as [C1 [C2 [A B]]]. 
-  subst. change C2 with (nil ++ C2). constructor. auto.
-Qed.
-
-Lemma match_config_skip:
-  forall C k m pc,
-  compile_cont C k pc ->
-  match_config C (SKIP, k, m) (pc, nil, m).
-Proof.
-  intros C.
-  assert (forall k pc, compile_cont C k pc -> codeseq_at C pc nil).
-    induction 1.
-    eapply code_at_codeseq; eauto.
-    change (compile_com c) with (nil ++ compile_com c) in H. eauto with codeseq.
-    eapply code_at_codeseq; eauto.
-    eapply code_at_codeseq; eauto.
-  intros. constructor. simpl. eauto. simpl. rewrite plus_0_r; auto.
-Qed.
-
-(** At long last, we can state and prove the right simulation diagram. *)
-
-Lemma simulation_step:
-  forall C impstate1 impstate2 machstate1,
-  kstep impstate1 impstate2 ->
-  match_config C impstate1 machstate1 ->
-  exists machstate2,
-      (plus (transition C) machstate1 machstate2
-       \/ (star (transition C) machstate1 machstate2 /\ measure impstate2 < measure impstate1))
-   /\ match_config C impstate2 machstate2.
-Proof.
-  intros until machstate1; intros KSTEP MATCH. 
-  inversion KSTEP; clear KSTEP; subst; inversion MATCH; clear MATCH; subst; simpl in *.
-
-- (* assign *)
-  econstructor; split.
-  left. eapply plus_right. eapply compile_aexp_correct; eauto with codeseq. 
-  eapply trans_setvar; eauto with codeseq. 
-  normalize. apply match_config_skip. auto.
-
-- (* seq *)
-  econstructor; split.
-  right; split. apply star_refl. omega. 
-  normalize. constructor. eauto with codeseq. eapply ccont_seq; eauto with codeseq. 
-
-- (* if true *)
-  set (code1 := compile_com c1) in *.
-  set (codeb := compile_bexp b false (length code1 + 1)) in *.
-  set (code2 := compile_com c2) in *.
-  econstructor; split.
-  right; split.
-  apply compile_bexp_correct with (b := b) (cond := false) (ofs := length code1 + 1).
-  eauto with codeseq.
-  omega.
-  rewrite H; simpl. fold codeb. normalize. constructor; eauto with codeseq. 
-  eapply ccont_branch; eauto with codeseq. 
-  change (S (length code2)) with (1 + length code2) in H5. normalize. auto.
-
-- (* if false *)
-  set (code1 := compile_com c1) in *.
-  set (codeb := compile_bexp b false (length code1 + 1)) in *.
-  set (code2 := compile_com c2) in *.
-  econstructor; split.
-  right; split.
-  apply compile_bexp_correct with (b := b) (cond := false) (ofs := length code1 + 1).
-  eauto with codeseq.
-  omega.
-  rewrite H; simpl. fold codeb. normalize. constructor; eauto with codeseq. 
-  change (S (length code2)) with (1 + length code2) in H5. normalize. auto.
-
-- (* while true *)
-  set (codec := compile_com c) in *.
-  set (codeb := compile_bexp b false (length codec + 1)) in *.
-  econstructor; split.
-  right; split.
-  apply compile_bexp_correct with (b := b) (cond := false) (ofs := length codec + 1).
-  eauto with codeseq.
-  omega.
-  rewrite H; simpl. fold codeb. normalize. constructor; eauto with codeseq.
-  fold codec.
-  assert (PC: pc + length codeb + length codec + 1 - (length codeb + length codec + 1) = pc)
-      by omega.
-  eapply ccont_while; eauto with codeseq. rewrite PC; auto. rewrite PC.
-  simpl. normalize. auto.
-
-- (* while false *)
-  set (codec := compile_com c) in *.
-  set (codeb := compile_bexp b false (length codec + 1)) in *.
-  econstructor; split.
-  right; split.
-  apply compile_bexp_correct with (b := b) (cond := false) (ofs := length codec + 1).
-  eauto with codeseq.
-  generalize (com_size_nonzero c). omega. 
-  rewrite H; simpl. fold codeb. normalize. apply match_config_skip. auto. 
-
-- (* skip seq *)
-  normalize.
-  destruct (compile_cont_Kseq_inv _ _ _ _ st H4) as [pc' [X [Y Z]]].
-  econstructor; split.
-  right; split. eexact X. omega.
-  constructor; auto. 
-
-- (* skip while *)
-  normalize.
-  destruct (compile_cont_Kwhile_inv _ _ _ _ _ st H4) as [pc' [X [Y Z]]].
-  econstructor; split.
-  left. eexact X. 
-  constructor; auto.
-Qed.
-
-(** Simulation diagrams such as [simulation_step] above imply semantic preservation
-  for terminating programs and for diverging programs.  We now develop a generic
-  proof of this fact that we can reuse later for other program transformations. *)
-
-Section SIMULATION_DIAGRAM.
-
-(** The generic proof is parameterized over the small-step semantics for the
-  source and target languages, and over an invariant between their states. *)
-
-Variable state1: Type.	     (**r the type of configurations for the source language *)
-Variable step1: state1 -> state1 -> Prop.   (**r the small-step semantics for the source language *)
-
-Variable state2: Type.	     (**r the type of configurations for the target language *)
-Variable step2: state2 -> state2 -> Prop.   (**r the small-step semantics for the target language *)
-
-Variable match_states: state1 -> state2 -> Prop.  (**r the invariant *)
-
-Variable measure: state1 -> nat.                  (**r the anti-stuttering measure *)
-
-Hypothesis simulation:
-  forall S1 S1' S2,
-  step1 S1 S1' -> match_states S1 S2 ->
-  exists S2',
-    (plus step2 S2 S2' \/ (star step2 S2 S2' /\ measure S1' < measure S1))
-  /\ match_states S1' S2'.
-
-(** We first extend the simulation to finite sequences of source transitions.
-  This will show semantic preservation for terminating programs. *)
-
-Lemma simulation_star:
-  forall S1 S1', star step1 S1 S1' ->
-  forall S2, match_states S1 S2 ->
-  exists S2', star step2 S2 S2' /\ match_states S1' S2'.
-Proof.
-  induction 1; intros.
-- (* zero transition *)
-  exists S2; split. apply star_refl. auto.
-- (* one or more transitions *)
-  destruct (simulation _ _ _ H H1) as [S2' [P Q]].
-  destruct (IHstar _ Q) as [S2'' [U V]].
-  exists S2''; split. 
-  eapply star_trans; eauto. destruct P. apply plus_star; auto. destruct H2; auto.
-  auto.
-Qed.
-
-(** Turning to infinite sequences, we first show that the target program
-  can always make progress, while preserving the [match_states] relation,
-  if the source diverges.  The proof is an induction on the maximal number
-  [N] of stutterings the target can make before performing at least one transition. *)
-
-Lemma simulation_infseq_productive:
-  forall N S1 S2,
-  measure S1 < N ->
-  infseq step1 S1 ->
-  match_states S1 S2 ->
-  exists S1', exists S2',
-      plus step2 S2 S2'
-   /\ infseq step1 S1'
-   /\ match_states S1' S2'.
-Proof.
-  induction N; intros. 
-- (* N = 0 *)
-  exfalso. omega.
-- (* N > 0 *)
-  inversion H0; clear H0; subst.
-  destruct (simulation _ _ _ H2 H1) as [S2' [P Q]].
-  destruct P.
-  + (* one or several transitions *)
-    exists b; exists S2'; auto.
-  + (* zero, one or several transitions *)
-    destruct H0. inversion H0; clear H0; subst.
-    * (* zero transitions *)
-      eapply IHN; eauto. omega.
-    * (* one or several transitions *)
-      exists b; exists S2'; split. eapply plus_left; eauto. auto.
-Qed.
-
-(** It follows that the target performs infinitely many transitions if
-  started in a configuration that matches a diverging source configuration. *)
-
-Lemma simulation_infseq:
-  forall S1 S2,
-  infseq step1 S1 ->
-  match_states S1 S2 ->
-  infseq step2 S2.
-Proof.
-  intros. 
-  apply infseq_coinduction_principle_2 with
-    (X := fun S2 => exists S1, infseq step1 S1 /\ match_states S1 S2).
-  intros. destruct H1 as [S [A B]]. 
-  destruct (simulation_infseq_productive (measure S + 1) S a) 
-  as [S1' [S2' [P [Q R]]]].
-  omega. auto. auto.
-  exists S2'; split. auto. exists S1'; auto. 
-  exists S1; auto.
-Qed.
-
-End SIMULATION_DIAGRAM.
-
-(** We now apply these results to the Imp compiler.  We first obtain
-  an alternate proof of semantic preservation for terminating Imp programs. *)
-
-Lemma match_config_initial:
-  forall c st,
-  match_config (compile_program c) (c, Kstop, st) (0, nil, st).
-Proof.
-  intros. constructor.
-  change (compile_program c) with (nil ++ compile_com c ++ Ihalt :: nil). constructor. auto.
-  simpl. unfold compile_program. constructor. apply code_at_app. auto.
-Qed.
-
-Theorem compile_program_correct_terminating_2:
-  forall c st st',
-  kterminates c st st' ->
-  mach_terminates (compile_program c) st st'.
-Proof.
-  intros.
-  assert (exists machconf2, 
-           star (transition (compile_program c)) (0, nil, st) machconf2
-           /\ match_config (compile_program c) (SKIP, Kstop, st') machconf2).
-  eapply simulation_star; eauto. eapply simulation_step. apply match_config_initial.
-  destruct H0 as [machconf2 [STAR MS]]. 
-  inversion MS; subst. simpl in *. normalize. 
-  destruct (compile_cont_Kstop_inv _ _ st' H5) as [pc' [A B]].
-  red. exists pc'; split. auto. eapply star_trans; eauto.
-Qed.
-
-(** More interestingly, we also prove semantic preservation for diverging
-  Imp programs. *)
-
-Theorem compile_program_correct_diverging:
-  forall c st,
-  kdiverges c st ->
-  mach_diverges (compile_program c) st.
-Proof.
-  intros; red; intros. 
-  eapply simulation_infseq with (match_states := match_config (compile_program c)); eauto.
-  eapply simulation_step. apply match_config_initial.
-Qed.
-
-(** *** Mini-project (4 stars) *)
-
-(** Our compiler for arithmetic expressions implements a left-to-right
-  evaluation order: in [a1 + a2], [a1] is evaluated first, and its value
-  left on the stack; then [a2] is evaluated; then an [Iadd] instruction
-  is performed.  For commutative operators like [+] and [*], we
-  could just as well evaluate [a2] first, then [a1], then combine
-  their results.  
-
-  This can help producing more efficient code in terms of how much
-  stack space is required by the evaluation.  Consider the expression
-  [1 + (2 + (3 + ... (N-1 + N)))].  With left-to-right evaluation,
-  it uses [N+1] stack entries.  With right-to-left evaluation,
-  it uses only 2 stack entries.  
-
-  In this exercise, we explore the effect of different evaluation orders
-  on stack usage.  Let us first parameterize [compile_aexp] with
-  a heuristic function [ord] that, given the two arguments of a [+]
-  or [*] operator, decides whether to evaluate them left-to-right
-  or right-to-left: *)
-
-Inductive eval_order : Type := LtoR | RtoL.
-
-Fixpoint compile_aexp_gen (ord: aexp -> aexp -> eval_order) (a: aexp) : code :=
+Fixpoint compile_aexp (stklen: nat) (vlist : varlist) (a:aexp): code :=
   match a with
   | ANum n => Iconst n :: nil
-  | AId v => Ivar v :: nil
-  | APlus a1 a2 =>
-      match ord a1 a2 with
-      | LtoR => compile_aexp_gen ord a1 ++ compile_aexp_gen ord a2 ++ Iadd :: nil
-      | RtoL => compile_aexp_gen ord a2 ++ compile_aexp_gen ord a1 ++ Iadd :: nil
-      end
-  | AMinus a1 a2 =>
-      compile_aexp_gen ord a1 ++ compile_aexp_gen ord a2 ++ Isub :: nil
-  | AMult a1 a2 =>
-      match ord a1 a2 with
-      | LtoR => compile_aexp_gen ord a1 ++ compile_aexp_gen ord a2 ++ Imul :: nil
-      | RtoL => compile_aexp_gen ord a2 ++ compile_aexp_gen ord a1 ++ Imul :: nil
-      end
+  | AId x => match find x vlist with
+             | None => Iconst 0 :: nil
+             | Some n => Iget (stklen-(length vlist)+n) :: nil
+             end
+  | APlus a1 a2 => let code1 := compile_aexp stklen vlist a1 in
+                   let code2 := compile_aexp (stklen+1) vlist a2 in
+                   code1 ++ code2 ++ Iadd::nil
+  | AMul a1 a2 => let code1 := compile_aexp stklen vlist a1 in
+                   let code2 := compile_aexp (stklen+1) vlist a2 in
+                   code1 ++ code2 ++ Imul::nil
+  | AMinus a1 a2 => let code1 := compile_aexp stklen vlist a1 in
+                   let code2 := compile_aexp (stklen+1) vlist a2 in
+                   code1 ++ code2 ++ Isub::nil
   end.
 
-(** First show that, whatever the [ord] heuristic is, the code generated
-by [compile_aexp_gen ord] is correct.  This is a simple extension of
-the proof of [compile_aexp_correct]. *)
 
-Lemma compile_aexp_gen_correct:
-  forall ord C st a pc stk,
-  codeseq_at C pc (compile_aexp_gen ord a) ->
+Fixpoint compile_bexp (stklen: nat) (vlist : varlist) (b:bexp) (cond:bool) (ofs:nat): code :=
+  match b with
+  | BTrue => if cond then Ibranch_forward ofs :: nil else nil
+  | BFalse => if cond then nil else Ibranch_forward ofs :: nil
+  | BEq a1 a2 =>
+    let code1 := compile_aexp stklen vlist a1 in
+    let code2 := compile_aexp (stklen+1) vlist a2 in
+    code1 ++ code2 ++
+               (if cond then Ibeq ofs :: nil else Ibne ofs :: nil)
+  | BLe a1 a2 =>
+    let ans1 := compile_aexp stklen vlist a1 in
+    let ans2 := compile_aexp (stklen+1) vlist a2 in
+    ans1 ++ ans2 ++
+               (if cond then Ible ofs :: nil else Ibgt ofs :: nil)
+  | BNot b1 =>
+    compile_bexp stklen vlist b1 (negb cond) ofs
+  | BAnd b1 b2 =>
+    let code2 := compile_bexp stklen vlist b2 cond ofs in
+    let code1 := compile_bexp stklen vlist b1 false (if cond then length code2
+                                     else ofs + (length code2)) in
+     code1 ++ code2
+  end.
+
+
+Fixpoint compile_com (stklen : nat) (vlist: varlist) (c:com): code :=
+  match c with
+  | SKIP => nil
+  | c1 ;; c2 => (compile_com stklen
+                   vlist c1) ++ (compile_com stklen vlist c2)
+  | IFB b THEN ifso ELSE ifnot FI =>
+    let code_ifso := compile_com stklen vlist ifso in
+    let code_ifnot := compile_com stklen vlist ifnot in
+    compile_bexp stklen vlist b false (length code_ifso + 1)
+                 ++ code_ifso
+                 ++ Ibranch_forward (length code_ifnot)
+                 :: code_ifnot
+  | WHILE b DO body END =>
+    let code_body := compile_com stklen vlist body in
+    let code_test := compile_bexp stklen vlist b false (length code_body + 1) in
+    code_test
+      ++ code_body
+      ++ Ibranch_backward (length code_test + length code_body + 1)
+      :: nil
+  | var ::= a =>
+            match find (Id var) vlist with
+            | Some n =>
+              compile_aexp stklen vlist a
+                           ++ Iset (stklen - length vlist + n) ::nil
+            | _ => nil
+            end
+  end.
+
+
+Fixpoint initialize_vars (l : varlist): code :=
+  match l with
+  | nil => nil
+  | v :: l' => (Iconst O) :: initialize_vars l'
+  end.
+
+
+Fixpoint zerostk_of_len (n: nat) : stack :=
+  match n with | O => nil | S n' => O :: zerostk_of_len n' end.
+
+Definition compile_program (p: com): code :=
+  let vlist := gen_vlist p nil in
+  initialize_vars vlist
+  ++ compile_com (length vlist) vlist p
+  ++ Ihalt::nil.
+
+
+Fixpoint aeval (st : state) (a:aexp): nat :=
+  match a with
+  | ANum n => n
+  | AId x => st x
+  | APlus a1 a2 => (aeval st a1) + (aeval st a2)
+  | AMinus a1 a2 => (aeval st a1) - (aeval st a2)
+  | AMul a1 a2 => (aeval st a1) * (aeval st a2)
+  end.
+
+
+Fixpoint beval (st : state) (b : bexp) : bool :=
+  match b with
+  | BTrue       => true
+  | BFalse      => false
+  | BEq a1 a2   => beq_nat (aeval st a1) (aeval st a2)
+  | BLe a1 a2   => leb (aeval st a1) (aeval st a2)
+  | BNot b1     => negb (beval st b1)
+  | BAnd b1 b2  => andb (beval st b1) (beval st b2)
+  end.
+
+
+
+Fixpoint aeval_stk (v:varlist) (stk: stack) (a:aexp): nat :=
+  match a with
+  | ANum n => n
+  | AId x => match find x v with
+             | Some n =>
+               match get_nth_slot stk ((length stk) - (length v) + n) with
+               | Some val => val
+               | _ => 0
+               end
+             | _ => 0
+             end
+  | APlus a1 a2 => (aeval_stk v stk a1) + (aeval_stk v ((aeval_stk v stk a1) ::stk) a2)
+  | AMinus a1 a2 => (aeval_stk v stk a1) - (aeval_stk v ((aeval_stk v stk a1) ::stk) a2)
+  | AMul a1 a2 => (aeval_stk v stk a1) * (aeval_stk v ((aeval_stk v stk a1) ::stk) a2)
+  end.
+
+Fixpoint beval_stk (v:varlist) (stk: stack) (b:bexp): bool :=
+  match b with
+  | BTrue => true
+  | BFalse => false
+  | BEq a1 a2 => beq_nat (aeval_stk v stk a1) (aeval_stk v stk a2)
+  | BLe a1 a2 => leb (aeval_stk v stk a1) (aeval_stk v stk a2)
+  | BNot b1 => negb (beval_stk v stk b1)
+  | BAnd b1 b2 => andb (beval_stk v stk b1) (beval_stk v stk b2)
+  end.
+
+
+
+Inductive varlist_contains_all : com -> varlist -> Prop :=
+| Vseq : forall c1 c2 vlist,
+    varlist_contains_all c1 vlist ->
+    varlist_contains_all c2 vlist ->
+    varlist_contains_all (c1 ;; c2) vlist
+| Vifb : forall c1 c2 vlist b,
+    varlist_contains_all c1 vlist ->
+    varlist_contains_all c2 vlist ->
+    varlist_contains_all (IFB b THEN c1 ELSE c2 FI) vlist
+| Vwhile: forall c vlist b,
+    varlist_contains_all c vlist ->
+    varlist_contains_all (WHILE b DO c END) vlist
+| Vskip : forall vlist, varlist_contains_all SKIP vlist
+| Vass : forall  vlist x a,
+    (exists n, find (Id x) vlist = Some n) ->
+    varlist_contains_all (x ::= a) vlist.
+
+
+
+Theorem extend_gen_vlist:
+  forall a x l,
+    varlist_contains_all a l ->
+    varlist_contains_all a (x::l).
+Proof.
+  induction a.
+  - constructor.
+  - intros. inversion H. subst.
+    apply Vass.
+    destruct (if string_dec x0 x then true else false) eqn:E.
+    + simpl. rewrite E.  exists 0. reflexivity.
+    + simpl. rewrite E. destruct H3. rewrite H0. exists (S x1).
+      reflexivity.
+  - intros. inversion H. subst. apply Vseq; auto.
+  - intros. inversion H. subst. apply Vifb; auto.
+  - intros. inversion H. subst. apply Vwhile. auto.
+Qed.
+
+Theorem gen_gen_vlist:
+  forall b a l ,
+    varlist_contains_all a l ->
+    varlist_contains_all a (gen_vlist b l).
+Proof.
+  induction b.
+  - simpl. auto.
+  - intros. simpl. destruct (find x l) eqn:E. assumption.
+    apply extend_gen_vlist. assumption.
+  - simpl. intros. cut (varlist_contains_all a (gen_vlist b1 l)); intuition.
+  - simpl. intros. cut (varlist_contains_all a (gen_vlist b2 l)); intuition.
+  - simpl. intros. auto.
+Qed.
+
+
+
+Theorem gen_vlist_contains_all :
+  forall c l, varlist_contains_all c (gen_vlist c l).
+Proof.
+  induction c.
+  - simpl. constructor.
+  - intros. simpl. apply Vass. simpl.
+    destruct (find x l) eqn:E.
+    + rewrite E. exists n. reflexivity. 
+    + simpl. rewrite string_dec_refl. exists 0. reflexivity.
+  - simpl. intros. apply Vseq. apply gen_gen_vlist. auto. auto.
+  - simpl. intros. apply Vifb. apply gen_gen_vlist. auto. auto.
+  - simpl. intros. apply Vwhile. auto.
+Qed.
+
+
+Definition agree (v : varlist) (stk : stack) (st : state) :=
+  length stk = length v /\
+  (forall i,
+    (forall n, find i v = Some n ->
+               (get_nth_slot stk (length stk - length v + n) = Some (st i)) )
+    /\
+    (find i v = None -> st i = O))
+.
+
+
+Theorem aeval_stk_appended: forall (v : varlist) (a:aexp) (stk: stack) (s : nat) ,
+    length v <= length stk ->
+    aeval_stk v stk a = aeval_stk v (s::stk) a.
+Proof.
+  assert (G: forall (n s:nat) stk (v:varlist),
+             length stk >= length v ->
+             get_nth_slot (s :: stk) (length (s :: stk) - length v + n)
+             =
+             get_nth_slot stk (length stk - length v + n)). 
+  {
+    intros.
+    assert (t: length (s::stk) - length v = S (length stk - length v)).
+    { simpl. destruct (length v). omega. omega. }
+    rewrite t.
+    simpl. reflexivity.
+  }
+
+  induction a.
+  - simpl. reflexivity.
+  - intros. unfold aeval_stk.
+    destruct (find i v) eqn:E; try auto.
+    rewrite G. reflexivity. omega.
+  - intros. simpl. rewrite (IHa1 stk s H).
+    cut (aeval_stk v (aeval_stk v (s :: stk) a1 :: stk) a2 =
+         aeval_stk v (aeval_stk v (s :: stk) a1 :: s ::  stk) a2). omega.
+    assert (P1: aeval_stk v (s :: stk) a2 = aeval_stk v stk a2).
+    { symmetry. auto.  }
+    assert (P2: aeval_stk v (s :: stk) a2
+                =
+                aeval_stk v (aeval_stk v (s :: stk) a1 :: s :: stk) a2).
+    { apply IHa2. simpl. omega. }
+    
+    assert (P3: aeval_stk v (stk) a2
+                =
+                aeval_stk v (aeval_stk v (s :: stk) a1 :: stk) a2).
+    { apply IHa2. simpl. omega. }
+    omega.
+  - intros. simpl. rewrite (IHa1 stk s H).
+    cut (aeval_stk v (aeval_stk v (s :: stk) a1 :: stk) a2 =
+         aeval_stk v (aeval_stk v (s :: stk) a1 :: s ::  stk) a2). omega.
+    assert (P1: aeval_stk v (s :: stk) a2 = aeval_stk v stk a2).
+    { symmetry. auto.  }
+    assert (P2: aeval_stk v (s :: stk) a2
+                =
+                aeval_stk v (aeval_stk v (s :: stk) a1 :: s :: stk) a2).
+    { apply IHa2. simpl. omega. }
+    assert (P3: aeval_stk v (stk) a2
+                =
+                aeval_stk v (aeval_stk v (s :: stk) a1 :: stk) a2).
+    { apply IHa2. simpl. omega. }
+    omega.
+  - intros. simpl. rewrite (IHa1 stk s H).
+    cut (aeval_stk v (aeval_stk v (s :: stk) a1 :: stk) a2 =
+         aeval_stk v (aeval_stk v (s :: stk) a1 :: s ::  stk) a2).
+    intros.
+    rewrite H0. reflexivity.
+    assert (P1: aeval_stk v (s :: stk) a2 = aeval_stk v stk a2).
+    { symmetry. auto.  }
+    assert (P2: aeval_stk v (s :: stk) a2
+                =
+                aeval_stk v (aeval_stk v (s :: stk) a1 :: s :: stk) a2).
+    { apply IHa2. simpl. omega. }
+    assert (P3: aeval_stk v (stk) a2
+                =
+                aeval_stk v (aeval_stk v (s :: stk) a1 :: stk) a2).
+    { apply IHa2. simpl. omega. }
+    omega.  
+Qed.
+
+
+
+Fact agree_aeval (v : varlist) (stk : stack) (st: state) :
+  forall (a:aexp),
+    agree v stk st -> aeval st a = aeval_stk v stk a.
+Proof.
+  unfold agree.
+  induction a; intros; destruct H.
+  - reflexivity.
+
+  - simpl. destruct (H0 i).
+    destruct (find i v) eqn:E.
+    rewrite H1. auto. auto. auto.
+    
+  - simpl. rewrite IHa1. rewrite IHa2.
+    simpl. rewrite <- aeval_stk_appended. reflexivity. omega.
+    split. omega. intros. auto. auto.
+
+  - simpl. rewrite IHa1. rewrite IHa2.
+    simpl. rewrite <- aeval_stk_appended. reflexivity. omega.
+    split. omega. intros. auto. auto.
+
+  - simpl. rewrite IHa1. rewrite IHa2.
+    simpl. rewrite <- aeval_stk_appended. reflexivity. omega.
+    split. omega. intros. auto. auto.
+
+Qed.
+  
+Fact agree_beval (v : varlist) (stk : stack) (st: state) :
+  forall (b:bexp),
+    agree v stk st -> beval st b = beval_stk v stk b.
+Proof.
+  induction b; simpl; intros; eauto using agree_aeval.
+  - rewrite (IHb H). reflexivity.
+  - rewrite (IHb1 H). rewrite (IHb2 H). reflexivity.
+Qed.
+    
+Reserved Notation "c1 '/' st '\\' st'"
+                  (at level 40, st at level 39).
+
+Inductive ceval : com -> state -> state -> Prop :=
+  | E_Skip : forall st,
+      SKIP / st \\ st
+  | E_Ass  : forall st a1 n x,
+      aeval st a1 = n ->
+      (x ::= a1) / st \\ (t_update st (Id x) n)
+  | E_Seq : forall c1 c2 st st' st'',
+      c1 / st  \\ st' ->
+      c2 / st' \\ st'' ->
+      (c1 ;; c2) / st \\ st''
+  | E_IfTrue : forall st st' b c1 c2,
+      beval st b = true ->
+      c1 / st \\ st' ->
+      (IFB b THEN c1 ELSE c2 FI) / st \\ st'
+  | E_IfFalse : forall st st' b c1 c2,
+      beval st b = false ->
+      c2 / st \\ st' ->
+      (IFB b THEN c1 ELSE c2 FI) / st \\ st'
+  | E_WhileFalse : forall b st c,
+      beval st b = false ->
+      (WHILE b DO c END) / st \\ st
+  | E_WhileTrue : forall st st' st'' b c,
+      beval st b = true ->
+      c / st \\ st' ->
+      (WHILE b DO c END) / st' \\ st'' ->
+      (WHILE b DO c END) / st \\ st''
+
+  where "c1 '/' st '\\' st'" := (ceval c1 st st').
+
+
+
+
+
+Lemma compile_aexp_correct:
+  forall (a:aexp) (C:code) (stk:stack) (pc:nat) (vlist:varlist),
+    forall (ineq : length stk >= length vlist), 
+    codeseq_at C pc (compile_aexp (length stk) vlist a) ->
+    star (transition C) (pc, stk)
+         (pc + length(compile_aexp (length stk) vlist a),
+          (aeval_stk vlist stk a)::stk).
+Proof.
+  induction a.
+  - intros. apply star_one. apply trans_const. eauto with codeseq. 
+  - intros.
+    apply star_one.
+    simpl in *.
+    destruct (find i vlist) eqn:E.
+    + simpl. eapply trans_get. eauto with codeseq.
+      
+      destruct (find_get_ofs _ _ _  stk ineq E) as [m mH].
+      rewrite mH. reflexivity.
+    + simpl. apply trans_const. eauto with codeseq.
+  
+  - intros. simpl. eapply star_trans.
+    apply (IHa1 C stk pc vlist ineq). eauto with codeseq.
+    eapply star_trans. apply (IHa2 _ _ _ vlist). simpl. omega. simpl in H.
+    rewrite plus_comm in H. simpl in H. eauto with codeseq.
+    apply star_one. repeat (rewrite app_length || simpl).
+    rewrite plus_assoc. rewrite (Nat.add_1_r (length stk)).
+    rewrite plus_assoc with (p := 1).
+    apply trans_add. simpl in H. rewrite Nat.add_1_r in H. eauto with codeseq.
+  - intros. simpl. eapply star_trans.
+    apply (IHa1 C stk pc vlist ineq). eauto with codeseq.
+    eapply star_trans. apply (IHa2 _ _ _ vlist). simpl. omega. simpl in H.
+    rewrite plus_comm in H. simpl in H. eauto with codeseq.
+    apply star_one. repeat (rewrite app_length || simpl).
+    rewrite plus_assoc. rewrite (Nat.add_1_r (length stk)).
+    rewrite plus_assoc with (p := 1).
+    apply trans_sub. simpl in H. rewrite Nat.add_1_r in H. eauto with codeseq.
+  - intros. simpl. eapply star_trans.
+    apply (IHa1 C stk pc vlist ineq). eauto with codeseq.
+    eapply star_trans. apply (IHa2 _ _ _ vlist). simpl. omega. simpl in H.
+    rewrite plus_comm in H. simpl in H. eauto with codeseq.
+    apply star_one. repeat (rewrite app_length || simpl).
+    rewrite plus_assoc. rewrite (Nat.add_1_r (length stk)).
+    rewrite plus_assoc with (p := 1).
+    apply trans_mul. simpl in H. rewrite Nat.add_1_r in H. eauto with codeseq.
+  
+Qed.
+
+Lemma compile_bexp_correct:
+  forall (b:bexp) (C:code) (stk:stack) (pc:nat) (vlist:varlist) (cond:bool) (ofs:nat),
+    length stk >= length vlist ->
+    codeseq_at C pc (compile_bexp (length stk) vlist b cond ofs) ->
   star (transition C)
-       (pc, stk, st)
-       (pc + length (compile_aexp_gen ord a), aeval st a :: stk, st).
+       (pc, stk)
+       (pc + length (compile_bexp (length stk) vlist b cond ofs) +
+        if eqb (beval_stk vlist stk b) cond then ofs else 0, stk).
 Proof.
-  induction a; simpl; intros.
-  (* FILL IN HERE *)
-Admitted.
+  induction b.
+  - simpl in *. intros. destruct cond eqn:E.
+    apply star_one. eapply trans_branch_forward. eauto with codeseq.
+    simpl. auto. simpl. normalize. apply star_refl.
+  - simpl in *. intros. destruct cond; simpl.
+    normalize. apply star_refl.
+    apply star_one. eapply trans_branch_forward. eauto with codeseq. auto.
+  - intros. simpl in *.
+    destruct cond.
+    + simpl. eapply star_trans. apply compile_aexp_correct. apply H. eauto with codeseq.
+      eapply star_trans. apply compile_aexp_correct. simpl.
+      cut( S (Datatypes.length stk) >= Datatypes.length vlist). intros. apply H1. omega.
+      simpl. rewrite Nat.add_1_r in H0. eauto with codeseq. normalize.
+      apply star_one. eapply trans_beq. rewrite Nat.add_1_r in *. eauto with codeseq.
+      pose (av := aeval_stk_appended vlist a0 stk (aeval_stk vlist stk a)).
+      rewrite <- av.
+      destruct (aeval_stk vlist stk a =? aeval_stk vlist stk a0) eqn:E;
+        simpl; normalize2; reflexivity. omega.
+    + simpl. eapply star_trans. apply compile_aexp_correct. apply H. eauto with codeseq.
+      eapply star_trans. apply compile_aexp_correct. simpl.
+      cut( S (Datatypes.length stk) >= Datatypes.length vlist). intros. apply H1. omega.
+      simpl. rewrite Nat.add_1_r in H0. eauto with codeseq. normalize.
+      apply star_one. eapply trans_bne. rewrite Nat.add_1_r in *. eauto with codeseq.
+      pose (av := aeval_stk_appended vlist a0 stk (aeval_stk vlist stk a)).
+      rewrite <- av.
+      destruct (aeval_stk vlist stk a =? aeval_stk vlist stk a0) eqn:E;
+        simpl; normalize2; reflexivity. omega.
+  - intros. simpl in *.
+    destruct cond.
+    + simpl. eapply star_trans. apply compile_aexp_correct. apply H. eauto with codeseq.
+      eapply star_trans. apply compile_aexp_correct. simpl.
+      cut( S (Datatypes.length stk) >= Datatypes.length vlist). intros. apply H1. omega.
+      simpl. rewrite Nat.add_1_r in H0. eauto with codeseq. normalize.
+      apply star_one. eapply trans_ble. rewrite Nat.add_1_r in *. eauto with codeseq.
+      pose (av := aeval_stk_appended vlist a0 stk (aeval_stk vlist stk a)).
+      rewrite <- av.
+      destruct (aeval_stk vlist stk a <=? aeval_stk vlist stk a0) eqn:E;
+        simpl; normalize2; reflexivity. omega.
+    + simpl. eapply star_trans. apply compile_aexp_correct. apply H. eauto with codeseq.
+      eapply star_trans. apply compile_aexp_correct. simpl.
+      cut( S (Datatypes.length stk) >= Datatypes.length vlist). intros. apply H1. omega.
+      simpl. rewrite Nat.add_1_r in H0. eauto with codeseq. normalize.
+      apply star_one. eapply trans_bgt. rewrite Nat.add_1_r in *. eauto with codeseq.
+      pose (av := aeval_stk_appended vlist a0 stk (aeval_stk vlist stk a)).
+      rewrite <- av.
+      destruct (aeval_stk vlist stk a <=? aeval_stk vlist stk a0) eqn:E;
+        simpl; normalize2; reflexivity. omega.
+  - intros. simpl in *. eapply star_trans. apply IHb. apply H. eauto with codeseq.
+    destruct cond; simpl; destruct (beval_stk vlist stk b); simpl; apply star_refl. 
+  - intros. simpl in *.
+    destruct cond; normalize2.
+    + eapply star_trans. apply IHb1. apply H. eauto with codeseq.
+      destruct (beval_stk vlist stk b1); normalize2; try apply star_refl.
+      apply IHb2. auto. eauto with codeseq.
+    + eapply star_trans. apply IHb1. apply H. eauto with codeseq.
+      destruct (beval_stk vlist stk b1);repeat normalize2.
+      * apply IHb2. auto. eauto with codeseq. 
+      * set (pc1 := (pc +
+                     Datatypes.length
+                       (compile_bexp (Datatypes.length stk) vlist b1 false
+                                     (ofs + Datatypes.length
+                                              (compile_bexp (Datatypes.length stk)
+                                                            vlist b2 false ofs))) +
+                     ofs + Datatypes.length (compile_bexp (Datatypes.length stk) vlist
+                                                          b2 false ofs)))
+          in *.
+        set (pc2 := (pc +
+                     Datatypes.length
+                       (compile_bexp (Datatypes.length stk) vlist b1 false
+                                     (ofs + Datatypes.length
+                                              (compile_bexp (Datatypes.length stk)
+                                                            vlist b2 false ofs))) +
+                     Datatypes.length (compile_bexp (Datatypes.length stk)
+                                                    vlist b2 false ofs) + ofs))
+          in *.
+        assert (H' : pc1 = pc2).
+        { unfold pc1, pc2. omega.  }
+        rewrite H'.
+        apply star_refl.
+Qed.
 
-(** Now, let us try to compute the minimum number of stack entries
-  needed to evaluate an expression, regardless of the strategy used. *)
-
-Require Import Min Max.     (**r Libraries of lemmas about min and max *)
-
-Fixpoint stack_needs (a: aexp) : nat :=
-  match a with
-  | ANum n => 1
-  | AId v => 1
-  | APlus a1 a2 =>
-      let n1 := stack_needs a1 in
-      let n2 := stack_needs a2 in
-      min (max n1 (n2 + 1)) (max n2 (n1 + 1))
-  | AMinus a1 a2 =>
-      let n1 := stack_needs a1 in
-      let n2 := stack_needs a2 in
-      max n1 (n2 + 1)
-  | AMult a1 a2 =>
-      let n1 := stack_needs a1 in
-      let n2 := stack_needs a2 in
-      min (max n1 (n2 + 1)) (max n2 (n1 + 1))
-  end.
-
-(** This definition is a variation on the Strahler numbering of a tree.
-  Here are some intuitions.  Consider [APlus a1 a2].  If we
-  evaluate [a1] then [a2], we will need at least [stack_needs a1]
-  space for evaluating [a1], then [stack_needs a2 + 1] for [a2]:
-  plus one, because during the evaluation of [a2], the value of [a1]
-  sits in the stack.  So, our space usage is the max of these two
-  quantities.  But we can also choose the other evaluation order,
-  so our space usage is the min of the two max corresponding to the
-  two possible evaluation orders. *)
-
-(** To show that [stack_needs] is the minimal stack size required,
-  we can define the stack usage (number of stack entries needed) of
-  a given strategy [ord], the show that it is at least [stack_needs]. *)
-
-Fixpoint stack_usage (ord: aexp -> aexp -> eval_order) (a: aexp) : nat :=
-  match a with
-  | ANum n => 1
-  | AId v => 1
-  | APlus a1 a2 =>
-      match ord a1 a2 with
-      | LtoR => max (stack_usage ord a1) (stack_usage ord a2 + 1)
-      | RtoL => max (stack_usage ord a2) (stack_usage ord a1 + 1)
-      end
-  | AMinus a1 a2 =>
-      max (stack_usage ord a1) (stack_usage ord a2 + 1)
-  | AMult a1 a2 =>
-      match ord a1 a2 with
-      | LtoR => max (stack_usage ord a1) (stack_usage ord a2 + 1)
-      | RtoL => max (stack_usage ord a2) (stack_usage ord a1 + 1)
-      end
-  end.
-
-Lemma stack_needs_is_optimal:
-  forall ord a, stack_needs a <= stack_usage ord a.
-Proof.
-  (* FILL IN HERE *)
-Admitted.
-
-(** Useful tip: the tactic [zify; omega] works very well to prove
-    arithmetic properties involving min and max operators. *)
-
-(** An optimal strategy (with respect to stack usage) is to always
-  compute the biggest subexpression first: *)
-
-Definition optimal_ord (a1 a2: aexp) :=
-  if leb (stack_needs a2) (stack_needs a1) then LtoR else RtoL.
-
-Definition compile_aexp_optimal (a: aexp) : code :=
-  compile_aexp_gen optimal_ord a.
-
-(** The intuition is simple: if one of the arguments, say [a1], has
-  stack needs strictly less than the other, say [a2], evaluating [a1]
-  after [a2], with [a2]'s value as additional entry on the stack,
-  will use no more stack space than evaluating [a2].  So, evaluating
-  [a1 + a2] can be done with no extra space than evaluating just [a2].
-  This would not be the case if we started with [a1], then evaluated [a2]:
-  in this case, one more stack slot would be needed. 
-
-  If both arguments have the same stack needs, the two evaluation
-  orders use exactly the same amount of space, so it does not matter
-  which one we choose. *)
-
-(** We can show the optimality of the strategy by observing that 
-  its stack usage is the minimum predicted by [stack_needs]. *)
-
-Lemma stack_usage_optimal_ord:
-  forall a, stack_usage optimal_ord a = stack_needs a.
-Proof.
-  (* FILL IN HERE *)
-Admitted.  
-
-(** So far, we've reasoned informally on the stack usage of a particular
-  evaluation strategy.  Now, let us formally connect this reasoning with the
-  execution of the compiled code.  First, we need to instrument the
-  virtual machine so that it monitors its stack usage and goes wrong
-  if the stack size goes over a given maximum [maxstack]. *)
-
-Inductive checked_transition (C: code) (maxstack: nat) : configuration -> configuration -> Prop :=
-  | ctrans: forall pc stk s pc' stk' s',
-      transition C (pc, stk, s) (pc', stk', s') ->
-      length stk' <= maxstack ->
-      checked_transition C maxstack (pc, stk, s) (pc', stk', s').
-
-(** Now, we can state and prove the fact that the compiled code for
-  expression [a] with respect to a strategy [ord] execute safely
-  if at least [stack_usage ord a] stack entries are available. *)
-
-Lemma compile_aexp_gen_safe:
-  forall ord C maxstack st a pc stk,
-  codeseq_at C pc (compile_aexp_gen ord a) ->
-  length stk + stack_usage ord a <= maxstack ->
-  star (checked_transition C maxstack)
-       (pc, stk, st)
-       (pc + length (compile_aexp_gen ord a), aeval st a :: stk, st).
-Proof.
-  induction a; simpl; intros.
-Admitted.
-
-(** Moreover, the size [stack_usage ord a] is tight, in that there exists
-  a point in the execution of the compiled code for [a] where the stack
-  is at least that big. *)
-
-Lemma stack_usage_reached:
-  forall ord C st a pc stk,
-  codeseq_at C pc (compile_aexp_gen ord a) ->
-  exists pc', exists stk',
-  star (transition C) (pc, stk, st) (pc', stk', st)
-  /\ length stk' >= length stk + stack_usage ord a.
-Proof.
-  induction a; simpl; intros.
-  (* FILL IN HERE *)
-Admitted.
-
-(** **** Full project (5 stars) *)
-
-Module StorelessMachine.
-
-(** The purpose of this project is to retarget the IMP compiler to a
-  different, simpler virtual machine that has no store, just a stack
-  that also supports direct accesses, i.e. reading or modifying the
-  N-th entry of the stack.  Here is the instruction set of the machine:
-*)
-
-Inductive instruction: Type :=
-  | Iconst(n: nat)                 (**r push integer [n] on stack *)
-  | Iget(n: nat)                   (**r push the value of the [n]-th stack slot *)
-  | Iset(n: nat)                   (**r pop an integer, assign it to the [n]-th stack slot *)
-  | Iadd                           (**r pop [n2], pop [n1], push back [n1+n2] *)
-  | Isub                           (**r pop [n2], pop [n1], push back [n1-n2] *)
-  | Imul                           (**r pop [n2], pop [n1], push back [n1*n2] *)
-  | Ibranch_forward(ofs: nat)      (**r skip [ofs] instructions forward *)
-  | Ibranch_backward(ofs: nat)     (**r skip [ofs] instructions backward *)
-  | Ibeq(ofs: nat)                 (**r pop [n2], pop [n1], skip [ofs] forward if [n1=n2] *)
-  | Ibne(ofs: nat)                 (**r pop [n2], pop [n1], skip [ofs] forward if [n1<>n2] *)
-  | Ible(ofs: nat)                 (**r pop [n2], pop [n1], skip [ofs] forward if [n1<=n2] *)
-  | Ibgt(ofs: nat)                 (**r pop [n2], pop [n1], skip [ofs] forward if [n1>n2] *)
-  | Ihalt.                         (**r terminate execution successfully *)
-
-(** The only difference with the original virtual machine is that the
-  [Ivar] and [Isetvar] instructions (to access the store by
-  identifier) are gone and replaced by [Iget] and [Iset] instructions
-  (to access the stack by position). *)
-
-Definition code := list instruction.
-Definition stack := list nat.
-Definition configuration := (nat * stack)%type.
-
-Fixpoint code_at (C: code) (pc: nat) : option instruction :=
-  match C, pc with
-  | nil, _ => None
-  | i :: C', O => Some i
-  | i :: C', S pc' => code_at C' pc'
-  end.
-
-(** To give semantics to the [Iget] and [Iset] instructions, start by
-  defining two stack-manipulating functions, such that
-<<
-     get_nth_slot (v0 :: ... :: vN :: ...) N = Some vN
-     set_nth_slot (v0 :: ... :: vN :: ...) N v' = Some (v0 :: ... :: v' :: ...)
->>
-*)
-
-Definition get_nth_slot (s: stack) (n: nat) : option nat :=
-  None. (* FILL HERE *)
-
-Fixpoint set_nth_slot (s: stack) (n: nat) (v: nat) : option stack :=
-  None. (* FILL HERE *)
-
-(** Then, the semantics of the machine is given by the following transition
-  relation.  Note that machine states are just pairs of a program counter
-  and a stack.  Note also that many transitions are exactly those of
-  the original machine after erasing the store component of the state. *)
-
-Inductive transition (C: code): configuration -> configuration -> Prop :=
-  | trans_const: forall pc stk n,
-      code_at C pc = Some(Iconst n) ->
-      transition C (pc, stk) (pc + 1, n :: stk)
-  | trans_get: forall pc stk n v,
-      code_at C pc = Some(Iget n) ->
-      get_nth_slot stk n = Some v ->
-      transition C (pc, stk) (pc + 1, v :: stk)
-  | trans_set: forall pc stk n v stk',
-      code_at C pc = Some(Iset n) ->
-      set_nth_slot stk n v = Some stk' ->
-      transition C (pc, v :: stk) (pc + 1, stk')
-  | trans_add: forall pc stk n1 n2,
-      code_at C pc = Some(Iadd) ->
-      transition C (pc, n2 :: n1 :: stk) (pc + 1, (n1 + n2) :: stk)
-  | trans_sub: forall pc stk n1 n2,
-      code_at C pc = Some(Isub) ->
-      transition C (pc, n2 :: n1 :: stk) (pc + 1, (n1 - n2) :: stk)
-  | trans_mul: forall pc stk n1 n2,
-      code_at C pc = Some(Imul) ->
-      transition C (pc, n2 :: n1 :: stk) (pc + 1, (n1 * n2) :: stk)
-  | trans_branch_forward: forall pc stk ofs pc',
-      code_at C pc = Some(Ibranch_forward ofs) ->
-      pc' = pc + 1 + ofs ->
-      transition C (pc, stk) (pc', stk)
-  | trans_branch_backward: forall pc stk ofs pc',
-      code_at C pc = Some(Ibranch_backward ofs) ->
-      pc' = pc + 1 - ofs ->
-      transition C (pc, stk) (pc', stk)
-  | trans_beq: forall pc stk ofs n1 n2 pc',
-      code_at C pc = Some(Ibeq ofs) ->
-      pc' = (if beq_nat n1 n2 then pc + 1 + ofs else pc + 1) ->
-      transition C (pc, n2 :: n1 :: stk) (pc', stk)
-  | trans_bne: forall pc stk ofs n1 n2 pc',
-      code_at C pc = Some(Ibne ofs) ->
-      pc' = (if beq_nat n1 n2 then pc + 1 else pc + 1 + ofs) ->
-      transition C (pc, n2 :: n1 :: stk) (pc', stk)
-  | trans_ble: forall pc stk ofs n1 n2 pc',
-      code_at C pc = Some(Ible ofs) ->
-      pc' = (if leb n1 n2 then pc + 1 + ofs else pc + 1) ->
-      transition C (pc, n2 :: n1 :: stk) (pc', stk)
-  | trans_bgt: forall pc stk ofs n1 n2 pc',
-      code_at C pc = Some(Ibgt ofs) ->
-      pc' = (if leb n1 n2 then pc + 1 else pc + 1 + ofs) ->
-      transition C (pc, n2 :: n1 :: stk) (pc', stk).
 
 Definition mach_terminates (C: code) (stk_init stk_fin: stack) :=
   exists pc,
   code_at C pc = Some Ihalt /\
   star (transition C) (0, stk_init) (pc, stk_fin).
 
-(** Now it's your turn: define a compilation scheme from IMP programs
-    to machine code and prove its correctness w.r.t. terminating executions,
-    as stated below. *)
 
-Definition compile_program (c: com) : code := nil. (* FILL HERE *)
 
-Theorem compile_program_correct_terminating:
-  forall c st,
-  c / empty_state \\ st ->
-  exists stk,
-     mach_terminates (compile_program c) nil stk
-  /\ True.
-Proof.
-  (* Have fun! *)
-Admitted.
-
-(** The [True] above is to be replaced by some informative relation between
-  the final stack [stk] and the final store [st]. *)
-
-(** Some hints to get you started.  Clearly, we need to use a portion of
-  the stack to hold the current values for the program variables.  It may
-  seem impossible to represent a store (a function from identifiers to values,
-  giving gives values to infinitely many variables) as a stack (a finite
-  list of values).  However, only the variables that are ever assigned to
-  within the program need to be associated with a stack slot: all
-  other variables keep their initial value of 0 throughout the program
-  execution. *)
-
-(**  Hence, the first order of business is to construct a list of
-  variables that are ever assigned in the program, and, from this
-  list, to assign a position in the stack for every such variable.
-  For example, if the list of assigned variables is [["x";"y";"z"]]
-  we could say that the value of ["x"] is at the top of the stack,
-  the value of ["y"] one slot below, and that of ["z"] two slots below.
-  Those offsets need adjusting during the evaluation of expressions,
-  because intermediate results are pushed on the stack on top of the
-  values of variables. *)
-
-(**  Using this information, the compilation of an expression [AId id] is
-  either [Iconst 0] if the variable is not assigned in the program,
-  or, [Iget N] otherwise, for a stack distance [N] that reflects the
-  stack position of variable [id]. *)
-
-(** To state and prove semantic preservation for the compilation functions,
-  you will need a predicate [agree st stk] that relates an IMP store [st]
-  with a machine stack [stk].  Typically, it will say that
-- [st x = 0] for all non-assigned variables [x]
-- [get_nth_slot stk N = Some (st x)] if [N] is the stack offset for variable [x]
-
-  The predicate [agree st stk] acts both as a pre- and a post-condition, e.g.
-
-<<
 Lemma compile_com_correct_terminating:
-  forall C st c st',
-  c / st \\ st' ->
-  forall stk pc,
-  codeseq_at C pc (compile_com c) ->
-  agree st stk ->
+  forall (c : com) (st st': state),
+    c / st \\ st' ->
+    forall (C:code) (stk:stack) (vlist:varlist) (pc:nat),
+    varlist_contains_all c vlist ->
+    codeseq_at C pc (compile_com (length stk) vlist c) ->
+    agree vlist stk st ->
   exists stk',
-     star (transition C) (pc, stk) (pc + length (compile_com c), stk')
-  /\ agree st' stk'.
->>
-*)
+     star (transition C) (pc, stk) (pc + length (compile_com (length stk) vlist c), stk')
+     /\ agree vlist stk' st'.
+Proof.
+  induction 1.
+  {
+    intros.
+    exists stk. simpl. split. rewrite Nat.add_0_r. apply star_refl.
+    inversion H. subst. assumption.
+  }
+  {
+    intros. inversion H0. subst. clear H0. rename H6 into H0. destruct H0 as [m H0].
+    set ( n := aeval st a1). assert (H : n = aeval st a1). auto.
+    remember H2 as ag.
+    destruct H2 as [H2 H2'].
+    
+    assert (Nstk : exists stk', set_nth_slot stk m n = Some stk').
+    { apply set_nth_success. rewrite H2. eapply find_success_list_length. eauto. }
+    destruct Nstk as [stk' Nstk].
+    
+    eexists. simpl. normalize. rewrite H0 in *.
+    split.
+    {
+      eapply star_trans. apply compile_aexp_correct.
+      Search "ge".
+      assert (lenIneq : length stk >= length vlist). omega.
+      apply lenIneq.
+      eauto with codeseq.
+      apply star_one. normalize. eapply trans_set. eauto with codeseq.
+      rewrite H2. rewrite Nat.sub_diag. simpl.
+      Search "aeval".
+      rewrite <- (agree_aeval _ _ _ a1 ag). rewrite H. apply Nstk.
+    }
+    {
+      
+      
+      Search "set_".
+      assert (f: length stk' = length vlist).
+      {
+        rewrite <- H2.
+        symmetry.
+        eapply set_nth_length with (stk' := stk'). apply Nstk.
+      }
+      unfold agree. split. assumption.
+      intros. split.
+      - intros. unfold t_update.
+        destruct (H2' i) as [h2 h2'].
+        destruct (beq_id x i) eqn:E. try apply beq_id_true_iff in E. 
+        + rewrite <- E in H3. rewrite H0 in H3. inversion H3. rewrite <- H5.
+          Search "get_set".
+          eapply get_set_eq. rewrite f. rewrite Nat.sub_diag. simpl.
+          apply Nstk.
+        + rewrite f. rewrite H2 in h2.
+          Search "get_other".
+          rewrite <- (h2 n0 H3).
+          eapply get_other_set. apply Nstk.
+          rewrite Nat.sub_diag. simpl. apply beq_id_false_iff in E.
+          Search "find".
+          destruct (find_inj2 _ _ _ _ _ H0 H3) as [contra contra']. auto.
+      - intros. destruct (H2' i) as [h2 h2'].
+        unfold t_update.
+        destruct (beq_id x i) eqn:E; apply beq_id_true_iff in E || apply beq_id_false_iff in E.
+        + subst. rewrite H3 in H0. discriminate.
+        + auto.
+      
+    }
+  }
+  {
+    intros. simpl in *.
+    inversion H1. subst. rename H6 into h1. rename H8 into h2.
+    assert (C1: codeseq_at C pc (compile_com (Datatypes.length stk) vlist c1)).
+    {eauto with codeseq. }
+    assert (C2: codeseq_at C (pc+length (compile_com (Datatypes.length stk) vlist c1))
+                           (compile_com (Datatypes.length stk) vlist c2)).
+    {eauto with codeseq. }
+    
+    destruct (IHceval1 C stk vlist pc h1 C1 H3) as [stk' [ih1 ih1']].
+    remember ih1' as t.
+    destruct t as [ih1'' h1'''].
+    remember H3 as t.
+    destruct t as [H3' H3''].
+    assert (stkE: length stk' = length stk).
+    { omega. }
+    rewrite <- stkE in C2.
+    destruct (IHceval2 C stk' vlist _ h2 C2 ih1') as [stk'' [ih2 ih2']].    
+    eexists. split.
+    - eapply star_trans. apply ih1. normalize. repeat rewrite stkE in ih2. apply ih2.
+    - assumption.
+  }
+  {
+    intros. simpl in H2.
 
-End StorelessMachine.
+    assert (Ct : codeseq_at C pc
+       (compile_bexp (Datatypes.length stk) vlist b false
+                     (Datatypes.length (compile_com (Datatypes.length stk) vlist c1) + 1))).
+    { eauto with codeseq. }
+
+    set (code_test := (compile_bexp (Datatypes.length stk) vlist b false
+                                    (Datatypes.length
+                                       (compile_com (Datatypes.length stk) vlist c1) + 1)))
+      in *.
+    set (code_ifso := compile_com (length stk) vlist c1).
+    set (code_ifnot := compile_com (length stk) vlist c2).
+    
+    assert (C1 : codeseq_at C (pc + Datatypes.length code_test)
+                            (compile_com (Datatypes.length stk) vlist c1)). {eauto with codeseq. }
+    assert (C2: codeseq_at C (pc + length code_test + length code_ifso + 1) code_ifnot).
+    { eauto with codeseq. }
+
+    remember H3 as t. destruct t as [H3' H3'']. clear Heqt.
+    assert (Hineq : length stk >= length vlist). omega.
+    pose (btest := compile_bexp_correct b C stk pc vlist false
+                                        (length (code_ifso) + 1) Hineq Ct).
+    inversion H1. subst. rename H8 into H1'. clear H1. rename H9 into H1.
+    destruct (IHceval C stk _ _ H1' C1 H3) as [stk' [ih ih']].
+    
+    eexists. split.
+    Check agree_beval.
+    - eapply star_trans. apply btest. rewrite <- (agree_beval _ _ _ b H3). rewrite H. simpl.
+      fold code_ifso code_ifnot code_test in ih |- *. normalize.
+      eapply star_trans. apply ih.
+      apply star_one. unfold code_ifso. unfold code_ifnot. eapply trans_branch_forward.
+      eauto with codeseq. unfold code_ifso, code_test, code_ifnot. omega.
+    - assumption.
+  }
+  {
+    intros. simpl in H2.
+
+    assert (Ct : codeseq_at C pc
+       (compile_bexp (Datatypes.length stk) vlist b false
+                     (Datatypes.length (compile_com (Datatypes.length stk) vlist c1) + 1))).
+    { eauto with codeseq. }
+
+    set (code_test := (compile_bexp (Datatypes.length stk) vlist b false
+                                    (Datatypes.length
+                                       (compile_com (Datatypes.length stk) vlist c1) + 1)))
+      in *.
+    set (code_ifso := compile_com (length stk) vlist c1) in code_test.
+    set (code_ifnot := compile_com (length stk) vlist c2) in code_test.
+    
+    assert (C1 : codeseq_at C (pc + Datatypes.length code_test)
+                            (compile_com (Datatypes.length stk) vlist c1)). {eauto with codeseq. }
+    assert (C2: codeseq_at C (pc + length code_test + length code_ifso + 1) code_ifnot).
+    { eauto with codeseq. }
+
+    remember H3 as t. destruct t as [H3' H3'']. clear Heqt.
+    assert (Hineq : length stk >= length vlist). omega.
+    pose (btest := compile_bexp_correct b C stk pc vlist false
+                                        (length (code_ifso) + 1) Hineq Ct).
+    
+    inversion H1. subst. rename H8 into H1'. clear H1. rename H9 into H1.
+    destruct (IHceval C stk _ _ H1 C2 H3) as [stk' [ih ih']].
+
+    eexists. split.
+    Check agree_beval.
+    - eapply star_trans. apply btest. rewrite <- (agree_beval _ _ _ b H3). rewrite H. simpl.
+      fold code_ifso code_ifnot code_test in ih |- *. normalize.
+      rewrite <- Nat.add_1_l with (length code_ifnot). normalize. apply ih.
+    - assumption.
+  }
+  {
+    simpl in *. intros.
+    set (code_body := compile_com (Datatypes.length stk) vlist c) in *.
+    set (code_test := compile_bexp (Datatypes.length stk) vlist b false
+                                   (Datatypes.length code_body + 1)) in *.
+    assert (Cb : codeseq_at C (pc + length code_test)
+                             (compile_com (Datatypes.length stk) vlist c)).
+    { eauto with codeseq. }
+    assert (Ct : codeseq_at C pc (compile_bexp (Datatypes.length stk) vlist b false
+                                               (Datatypes.length code_body + 1))).
+    { eauto with codeseq. }
+
+    remember H2 as t. destruct t as [H2' H2'']. clear Heqt.
+    assert (Hineq : length stk >= length vlist). omega.
+    
+    pose (jump:= compile_bexp_correct  _ _ _ _ _ _ _ Hineq Ct).
+    rewrite <- (agree_beval _ _ _ b H2) in jump.
+    eexists.
+    split. 2 : apply H2.
+    normalize.
+    rewrite H in jump. simpl in jump. normalize.
+    fold code_test in jump. assumption.    
+  }
+  {
+    intros.
+    set (code_body := compile_com (Datatypes.length stk) vlist c) in *.
+    set (code_test := compile_bexp (Datatypes.length stk) vlist b false
+                                   (Datatypes.length code_body + 1)) in *.
+    assert (Cb : codeseq_at C (pc + length code_test)
+                             (compile_com (Datatypes.length stk) vlist c)).
+    { eauto with codeseq. }
+    assert (Ct : codeseq_at C pc (compile_bexp (Datatypes.length stk) vlist b false
+                                               (Datatypes.length code_body + 1))).
+    { eauto with codeseq. }
+
+    
+    remember H4 as t. destruct t as [H4' H4'']. clear Heqt.
+    assert (Hineq : length stk >= length vlist). omega.
+    
+    pose (jump:= compile_bexp_correct  _ _ _ _ _ _ _ Hineq Ct).
+
+    rewrite <- (agree_beval _ _ _ b H4) in jump.
+    simpl. fold code_body code_test.
+    inversion H2. subst. rename H2 into H2o. rename H8 into H2.
+    destruct (IHceval1 C stk vlist _ H2 Cb H4) as [stk' [ihb ihb']]. 
+    assert (V: varlist_contains_all (WHILE b DO c END) vlist).
+    {auto. }
+
+    assert (L : length stk' = length stk).
+    { destruct H4. destruct ihb'. omega. }          
+
+    pose (Ihc2 := IHceval2 C stk' _ pc V).
+    rewrite L in Ihc2.
+    destruct (Ihc2 H3 ihb') as [stk'' ihc].
+    eexists. split.
+    eapply star_trans. apply jump.
+    rewrite H. simpl. fold code_body code_test. normalize. simpl.
+    eapply star_trans. apply ihb. fold code_body code_test.
+    eapply star_trans. apply star_one. eapply trans_branch_backward. eauto with codeseq.
+    2 : {
+      fold code_body code_test in ihc. normalize.
+      apply ihc.
+    }
+    fold code_body code_test. normalize. omega.
+    apply ihc.
+  }
+Qed.
+
+
+(*)
+Lemma compile_program_correct_terminating:
+  forall (c : com) (st': state),
+    c / empty_state \\ st' ->
+    exists vlist stk',
+      (star (transition (compile_program c))
+            (0, []) (length (compile_program c), stk')
+      /\ agree vlist stk' st').
+Proof.
+  intros.
+  set (vlist := gen_vlist c []) in *.
+  set (C := compile_program c).
+  assert (H1: varlist_contains_all c vlist ).
+  { unfold vlist. apply gen_vlist_contains_all.  }
+  exists vlist. unfold compile_program. fold vlist.
+
+  pose (P := compile_com_correct_terminating c empty_state st' H C []
+                                             vlist 0 ).
+  unfold C, compile_program.
+  eapply compile_com_correct_terminating.
+*)
