Facts.v
@@ -1,0 +1,237 @@
+(** This file contains results about 
+[find], [codeseq_at], [code_at], [get_nth_slot] and [set_nth_slot]*)
+
+From Coq Require Export Strings.String.
+From Coq Require Export Arith.Arith.
+From Coq Require Export Lists.List.
+From Coq Require Export Bool.Bool.
+Require Import Omega.
+From StorelessMachine Require Import Maps.
+From StorelessMachine Require Import Imp.
+
+Lemma code_at_app:
+  forall i c2 c1 pc,
+  pc = length c1 ->
+  code_at (c1 ++ i :: c2) pc = Some i.
+Proof.
+  induction c1; simpl; intros; subst pc; auto.
+Qed.
+
+Lemma codeseq_at_head:
+  forall C pc i C',
+  codeseq_at C pc (i :: C') ->
+  code_at C pc = Some i.
+Proof.
+  intros. inversion H. simpl. apply code_at_app. auto.
+Qed.
+
+Lemma codeseq_at_tail:
+  forall C pc i C',
+  codeseq_at C pc (i :: C') ->
+  codeseq_at C (pc + 1) C'.
+Proof.
+  intros. inversion H. 
+  change (C1 ++ (i :: C') ++ C3)
+    with (C1 ++ (i :: nil) ++ C' ++ C3).
+  rewrite <- app_ass. constructor. rewrite app_length. auto.
+Qed. 
+
+Lemma codeseq_at_app_left:
+  forall C pc C1 C2,
+  codeseq_at C pc (C1 ++ C2) ->
+  codeseq_at C pc C1.
+Proof.
+  intros. inversion H. rewrite app_ass. constructor. auto.
+Qed.
+
+Lemma codeseq_at_app_right:
+  forall C pc C1 C2,
+  codeseq_at C pc (C1 ++ C2) ->
+  codeseq_at C (pc + length C1) C2.
+Proof.
+  intros. inversion H. rewrite app_ass. rewrite <- app_ass. constructor. rewrite app_length. auto.
+Qed.
+
+Lemma codeseq_at_app_right2:
+  forall C pc C1 C2 C3,
+  codeseq_at C pc (C1 ++ C2 ++ C3) ->
+  codeseq_at C (pc + length C1) C2.
+Proof.
+  intros. inversion H. repeat rewrite app_ass. rewrite <- app_ass. constructor. rewrite app_length. auto.
+Qed.
+
+Hint Resolve code_at_app codeseq_at_head codeseq_at_tail codeseq_at_app_left
+     codeseq_at_app_right codeseq_at_app_right2 Nat.add_0_r Nat.add_1_r
+     Nat.add_assoc Nat.add_comm :codeseq.
+
+
+
+Fact find_success_list_length:
+  forall vlist i n,
+    find i vlist = Some n -> n < length vlist.
+Proof.
+  induction vlist as [| v vl].
+  - intros. discriminate.
+  - destruct i as [i]. simpl. rewrite if_string_dec_eqb.
+    destruct (v =? i)%string eqn:E.
+    + intros. injection H. omega.
+    + destruct (find (Id i) vl) as [m|] eqn:Q.
+      intros. injection H.
+      pose (H1 := IHvl _ _ Q). omega.
+      intros. discriminate.
+Qed.
+
+
+
+Fact get_nth_success: forall stk u, u < length stk -> exists v,
+      get_nth_slot stk u = Some v.
+Proof.
+  induction stk.
+  simpl. intros. omega.
+  intros u.
+  destruct u.
+  - subst. intros.
+    exists a. reflexivity.
+  - simpl. intros. apply IHstk. omega.
+Qed.
+
+
+
+Theorem find_get_ofs: forall (i:id) vlist n stk,
+    length stk >= length vlist ->
+    find i vlist = Some n ->
+    exists m,
+      get_nth_slot stk (length stk - length vlist + n) = Some m.
+Proof.
+  intros.
+  apply find_success_list_length in H0.
+  apply get_nth_success.
+  omega.
+Qed.
+
+
+Theorem set_nth_success:
+  forall stk pos val,
+    pos < length stk ->
+  exists stk',
+      set_nth_slot stk pos val = Some stk'.
+Proof.
+  induction stk.
+  - intros. simpl in H. omega.
+  - intros. destruct pos as [| pos]. simpl. eauto.
+    simpl in H.
+    cut (pos < length stk). simpl. intros.
+    destruct (IHstk pos val H0) as [ stk' hstk'].
+    rewrite hstk'. eauto.
+    omega.
+Qed.
+
+
+Theorem get_set_eq : forall pos l l' val,
+    set_nth_slot l pos val = Some l' ->
+    get_nth_slot l' pos = Some val.
+Proof.
+  induction pos.
+  - destruct l.
+    + discriminate.
+    + intros. simpl in H. inversion H. subst. reflexivity.
+  - intros. destruct l; try discriminate.
+    simpl in H.
+    destruct (set_nth_slot l pos val) eqn:E; try discriminate.
+    inversion H. simpl. eapply IHpos. apply E.
+Qed.
+
+Theorem get_other_set : forall val l' l n' n,
+    set_nth_slot l n val = Some l' ->
+    n' <> n ->
+    get_nth_slot l' n' = get_nth_slot l n'.
+Proof.
+  induction l'.
+  - intros. induction l. reflexivity.
+    simpl in *. destruct n. discriminate.
+    destruct (set_nth_slot l n val); discriminate.
+  - intros.
+    destruct l. {simpl in *. discriminate. }
+    destruct n.
+    + simpl in H. inversion H. subst.
+      destruct n'. omega.
+      simpl. reflexivity.
+    + simpl in H.
+      destruct (set_nth_slot l n val) eqn:E; try discriminate.
+      inversion H. subst.
+      destruct n'.
+      * simpl. reflexivity.
+      * simpl. eapply IHl'. apply E.
+        omega.
+Qed.
+
+Fact set_nth_length: forall stk' stk p v,
+    set_nth_slot stk p v = Some stk' ->
+    length stk = length stk'.
+Proof.
+  induction stk'.
+  - intros. simpl in H.
+    destruct stk; simpl in *. discriminate.
+    destruct p. discriminate. destruct (set_nth_slot stk p v); discriminate.
+  - intros. destruct stk.
+    + simpl in *. discriminate.
+    + simpl. destruct p; simpl in *. inversion H. subst. reflexivity.
+      destruct (set_nth_slot stk p v) eqn:E; try discriminate.
+      inversion H. subst. eauto.
+Qed.
+
+Theorem find_inj :
+  forall x y vl n,
+    find x vl = Some n ->
+    (find y vl = find x vl <-> x = y).
+Proof.
+  induction vl.
+  {intros. split; intros; simpl in *; discriminate. }
+  intros. split;intros.
+  destruct (beq_id a x) eqn:E.
+  - simpl in H. remember E as t. unfold beq_id in t. rewrite t in H.
+    inversion H. clear Heqt t. rewrite beq_id_true_iff in E. subst.
+    simpl in H0. rewrite string_dec_refl in H0.
+    destruct (beq_id a y) eqn:E.
+    + apply beq_id_true_iff in E. assumption.
+    + unfold beq_id in E. rewrite E in H0. destruct (find y vl); discriminate.
+  - destruct x as [ x'].
+    unfold beq_id in E.
+    destruct (beq_id a y) eqn:E'.
+    + apply beq_id_true_iff in E'. rewrite H in H0.
+      destruct y as [y'].
+      simpl in H0. inversion E'. clear E'.
+      rewrite H2 in H0. rewrite string_dec_refl in H0. inversion H0.
+      subst.
+      simpl in H.
+      destruct (if string_dec y' x' then true else false); try discriminate.
+      destruct (find x' vl); discriminate.
+    + destruct (if string_dec a x' then true else false) eqn:Ex; try discriminate.
+      * clear E. destruct y  as [y']. unfold beq_id in E'.
+        rewrite H in H0. simpl in H, H0. rewrite Ex in H. rewrite E' in H0.
+        destruct (find x' vl); try discriminate.
+        destruct (find y' vl); try discriminate.
+        inversion H. inversion H0.
+        eapply IHvl. destruct n. discriminate.
+        auto. rewrite <- H2 in H3. auto.
+  - subst. reflexivity.
+Qed.
+
+Theorem find_inj2 :
+  forall vl x y n1 n2,
+    find x vl = Some n1 ->
+    find y vl = Some n2 ->
+    (x = y <-> n1 = n2).
+Proof.
+  intros. split; intros.
+  - subst. rewrite H in H0. inversion H0. reflexivity.
+  - pose (Inj := find_inj _ y _ _ H).
+    rewrite <- Inj. rewrite <- H1 in H0. rewrite H0. auto.
+Qed.
+
+
+
+
+
+
+
